<?xml version="1.0"?>
<rdf:RDF xmlns="https://burbachs.github.io/AISHIPOntology/AISHIP#"
     xml:base="https://burbachs.github.io/AISHIPOntology/AISHIP"
     xmlns:dc="http://purl.org/dc/elements/1.1/"
     xmlns:owl="http://www.w3.org/2002/07/owl#"
     xmlns:rdf="http://www.w3.org/1999/02/22-rdf-syntax-ns#"
     xmlns:xml="http://www.w3.org/XML/1998/namespace"
     xmlns:xsd="http://www.w3.org/2001/XMLSchema#"
     xmlns:bibo="http://purl.org/ontology/bibo/"
     xmlns:foaf="http://xmlns.com/foaf/0.1/"
     xmlns:rdfs="http://www.w3.org/2000/01/rdf-schema#"
     xmlns:terms="http://purl.org/dc/terms/">
    <owl:Ontology rdf:about="https://burbachs.github.io/AISHIPOntology/AISHIP">
        <owl:imports rdf:resource="http://qudt.org/3.1.2/schema/qudt"/>
        <owl:imports rdf:resource="http://www.w3.org/1999/02/22-rdf-syntax-ns#Ontology"/>
        <terms:bibliographicCitation>Simon Burbach, Lennart Mackert, Maria Maleshkova (2025): AISHIP Ontology. https://doi.org/10.5281/zenodo.16704863</terms:bibliographicCitation>
        <terms:created rdf:datatype="http://www.w3.org/2001/XMLSchema#date">2025-07-23</terms:created>
        <terms:creator rdf:nodeID="genid1"/>
        <terms:creator rdf:nodeID="genid3"/>
        <terms:creator rdf:nodeID="genid5"/>
        <terms:license rdf:resource="https://creativecommons.org/licenses/by-nc-sa/4.0/"/>
        <terms:title>AISHIP Ontology</terms:title>
        <bibo:doi>10.5281/zenodo.16704863</bibo:doi>
        <rdfs:comment xml:lang="en">AISHIP is an ontology designed to enable semantic integration and enrichment of heterogeneous maritime data. It extends the VesselAI ontology with enhanced vessel characteristics, detailed propulsion systems, extended trajectory modeling, and multimodal vessel representations.</rdfs:comment>
    </owl:Ontology>
    <rdf:Description rdf:nodeID="genid1"/>
    <rdf:Description rdf:nodeID="genid3"/>
    <rdf:Description rdf:nodeID="genid5"/>
    


    <!-- 
    ///////////////////////////////////////////////////////////////////////////////////////
    //
    // Annotation properties
    //
    ///////////////////////////////////////////////////////////////////////////////////////
     -->


    


    <!-- http://purl.org/dc/terms/bibliographicCitation -->


    <owl:AnnotationProperty rdf:about="http://purl.org/dc/terms/bibliographicCitation"/>
    


    <!-- http://purl.org/dc/terms/created -->


    <owl:AnnotationProperty rdf:about="http://purl.org/dc/terms/created"/>
    


    <!-- http://purl.org/dc/terms/creator -->


    <owl:AnnotationProperty rdf:about="http://purl.org/dc/terms/creator"/>
    


    <!-- http://purl.org/dc/terms/license -->


    <owl:AnnotationProperty rdf:about="http://purl.org/dc/terms/license"/>
    


    <!-- http://purl.org/dc/terms/title -->


    <owl:AnnotationProperty rdf:about="http://purl.org/dc/terms/title"/>
    


    <!-- http://purl.org/ontology/bibo/doi -->


    <owl:AnnotationProperty rdf:about="http://purl.org/ontology/bibo/doi"/>
    


    <!-- http://xmlns.com/foaf/0.1/homepage -->


    <owl:AnnotationProperty rdf:about="http://xmlns.com/foaf/0.1/homepage"/>
    


    <!-- http://xmlns.com/foaf/0.1/mbox -->


    <owl:AnnotationProperty rdf:about="http://xmlns.com/foaf/0.1/mbox"/>
    


    <!-- http://xmlns.com/foaf/0.1/name -->


    <owl:AnnotationProperty rdf:about="http://xmlns.com/foaf/0.1/name"/>
    


    <!-- 
    ///////////////////////////////////////////////////////////////////////////////////////
    //
    // Datatypes
    //
    ///////////////////////////////////////////////////////////////////////////////////////
     -->


    


    <!-- http://www.w3.org/2001/XMLSchema#date -->


    <rdfs:Datatype rdf:about="http://www.w3.org/2001/XMLSchema#date"/>
    


    <!-- http://www.w3.org/2001/XMLSchema#gYear -->


    <rdfs:Datatype rdf:about="http://www.w3.org/2001/XMLSchema#gYear"/>
    


    <!-- 
    ///////////////////////////////////////////////////////////////////////////////////////
    //
    // Object Properties
    //
    ///////////////////////////////////////////////////////////////////////////////////////
     -->


    


    <!-- http://qudt.org/schema/qudt/unit -->


    <owl:ObjectProperty rdf:about="http://qudt.org/schema/qudt/unit"/>
    


    <!-- http://www.vesselAI-project.eu/ontology#hasGeometry -->


    <owl:ObjectProperty rdf:about="http://www.vesselAI-project.eu/ontology#hasGeometry"/>
    


    <!-- https://burbachs.github.io/AISHIPOntology/AISHIP#computedOverTimeInterval -->


    <owl:ObjectProperty rdf:about="https://burbachs.github.io/AISHIPOntology/AISHIP#computedOverTimeInterval">
        <rdfs:domain rdf:resource="https://burbachs.github.io/AISHIPOntology/AISHIP#TypicalLocation"/>
        <rdfs:range rdf:resource="http://www.w3.org/2006/time#Interval"/>
        <rdfs:comment xml:lang="en">Relatesa typical location with the time interval it was computed over.</rdfs:comment>
        <rdfs:label xml:lang="en">computed over time interval</rdfs:label>
    </owl:ObjectProperty>
    


    <!-- https://burbachs.github.io/AISHIPOntology/AISHIP#drivenBy -->


    <owl:ObjectProperty rdf:about="https://burbachs.github.io/AISHIPOntology/AISHIP#drivenBy">
        <owl:inverseOf rdf:resource="https://burbachs.github.io/AISHIPOntology/AISHIP#drives"/>
        <rdfs:domain rdf:resource="https://burbachs.github.io/AISHIPOntology/AISHIP#MotorizedPropulsionSystem"/>
        <rdfs:range rdf:resource="https://schema.org/EngineSpecification"/>
        <rdfs:comment xml:lang="en">Relates a motorized propulsion technology with the engine it is driven by.</rdfs:comment>
        <rdfs:label xml:lang="en">driven by</rdfs:label>
    </owl:ObjectProperty>
    


    <!-- https://burbachs.github.io/AISHIPOntology/AISHIP#drives -->


    <owl:ObjectProperty rdf:about="https://burbachs.github.io/AISHIPOntology/AISHIP#drives">
        <rdfs:domain rdf:resource="https://schema.org/EngineSpecification"/>
        <rdfs:range rdf:resource="https://burbachs.github.io/AISHIPOntology/AISHIP#MotorizedPropulsionTechnology"/>
        <rdfs:comment xml:lang="en">Relates an engine to the motorized propulsion technology it drives.</rdfs:comment>
        <rdfs:label xml:lang="en">drives</rdfs:label>
    </owl:ObjectProperty>
    


    <!-- https://burbachs.github.io/AISHIPOntology/AISHIP#hasActualHeight -->


    <owl:ObjectProperty rdf:about="https://burbachs.github.io/AISHIPOntology/AISHIP#hasActualHeight">
        <rdfs:domain rdf:resource="http://www.vesselAI-project.eu/ontology#Vessel"/>
        <rdfs:range>
            <owl:Class>
                <owl:intersectionOf rdf:parseType="Collection">
                    <rdf:Description rdf:about="http://qudt.org/schema/qudt/QuantityValue"/>
                    <owl:Restriction>
                        <owl:onProperty rdf:resource="http://qudt.org/schema/qudt/unit"/>
                        <owl:hasValue rdf:resource="https://qudt.org/3.1.2/vocab/unitM"/>
                    </owl:Restriction>
                    <owl:Restriction>
                        <owl:onProperty rdf:resource="http://qudt.org/schema/qudt/numericValue"/>
                        <owl:allValuesFrom rdf:resource="http://www.w3.org/2001/XMLSchema#decimal"/>
                    </owl:Restriction>
                </owl:intersectionOf>
            </owl:Class>
        </rdfs:range>
        <rdfs:comment xml:lang="en">Relates a vessel to its actual height. Indicates the actual current height of the vessel, e.g., considering load or structural changes, expressed in meters. Note: This property is semantically the same as http://www.vesselAI-project.eu/ontology#hasActualHeight. However, we allow the expression as a quantity with numeric value and a unit.</rdfs:comment>
        <rdfs:label xml:lang="en">has actual height</rdfs:label>
    </owl:ObjectProperty>
    


    <!-- https://burbachs.github.io/AISHIPOntology/AISHIP#hasAntiCavitationMechanism -->


    <owl:ObjectProperty rdf:about="https://burbachs.github.io/AISHIPOntology/AISHIP#hasAntiCavitationMechanism">
        <owl:inverseOf rdf:resource="https://burbachs.github.io/AISHIPOntology/AISHIP#isAntiCavitationMechanismFor"/>
        <rdfs:domain rdf:resource="https://burbachs.github.io/AISHIPOntology/AISHIP#MotorizedPropulsionTechnology"/>
        <rdfs:range rdf:resource="https://burbachs.github.io/AISHIPOntology/AISHIP#AntiCavitationMechanism"/>
        <rdfs:comment xml:lang="en">Relates a motorized propulsion technology to its anti-cavitation mechanism that reduces its cavitation.</rdfs:comment>
        <rdfs:label xml:lang="en">has anti-cavitation mechanism</rdfs:label>
    </owl:ObjectProperty>
    


    <!-- https://burbachs.github.io/AISHIPOntology/AISHIP#hasAverageSpeedOverGround -->


    <owl:ObjectProperty rdf:about="https://burbachs.github.io/AISHIPOntology/AISHIP#hasAverageSpeedOverGround">
        <rdfs:domain rdf:resource="http://www.vesselAI-project.eu/ontology#Vessel"/>
        <rdfs:range>
            <owl:Class>
                <owl:intersectionOf rdf:parseType="Collection">
                    <rdf:Description rdf:about="http://qudt.org/schema/qudt/QuantityValue"/>
                    <owl:Restriction>
                        <owl:onProperty rdf:resource="http://qudt.org/schema/qudt/unit"/>
                        <owl:hasValue rdf:resource="https://qudt.org/3.1.2/vocab/unitKN"/>
                    </owl:Restriction>
                    <owl:Restriction>
                        <owl:onProperty rdf:resource="http://qudt.org/schema/qudt/numericValue"/>
                        <owl:allValuesFrom rdf:resource="http://www.w3.org/2001/XMLSchema#decimal"/>
                    </owl:Restriction>
                </owl:intersectionOf>
            </owl:Class>
        </rdfs:range>
        <rdfs:comment xml:lang="en">Relates a vessel with its overall average speed over ground, typically measured in knots (kn).</rdfs:comment>
        <rdfs:label xml:lang="en">has average speed over ground</rdfs:label>
    </owl:ObjectProperty>
    


    <!-- https://burbachs.github.io/AISHIPOntology/AISHIP#hasAverageTrajectorySpeedOverGround -->


    <owl:ObjectProperty rdf:about="https://burbachs.github.io/AISHIPOntology/AISHIP#hasAverageTrajectorySpeedOverGround">
        <rdfs:domain rdf:resource="http://www.vesselAI-project.eu/ontology#Trajectory"/>
        <rdfs:range>
            <owl:Class>
                <owl:intersectionOf rdf:parseType="Collection">
                    <rdf:Description rdf:about="http://qudt.org/schema/qudt/QuantityValue"/>
                    <owl:Restriction>
                        <owl:onProperty rdf:resource="http://qudt.org/schema/qudt/unit"/>
                        <owl:hasValue rdf:resource="https://qudt.org/3.1.2/vocab/unitKN"/>
                    </owl:Restriction>
                    <owl:Restriction>
                        <owl:onProperty rdf:resource="http://qudt.org/schema/qudt/numericValue"/>
                        <owl:allValuesFrom rdf:resource="http://www.w3.org/2001/XMLSchema#decimal"/>
                    </owl:Restriction>
                </owl:intersectionOf>
            </owl:Class>
        </rdfs:range>
        <rdfs:comment xml:lang="en">Relates a trajtectory to the average speed over ground of the vessel during that trip, typically measured in knots (kn).</rdfs:comment>
        <rdfs:label xml:lang="en">has average trajectory speed over ground</rdfs:label>
    </owl:ObjectProperty>
    


    <!-- https://burbachs.github.io/AISHIPOntology/AISHIP#hasCourseOverGround -->


    <owl:ObjectProperty rdf:about="https://burbachs.github.io/AISHIPOntology/AISHIP#hasCourseOverGround">
        <rdfs:domain rdf:resource="http://www.vesselAI-project.eu/ontology#Vessel"/>
        <rdfs:range>
            <owl:Class>
                <owl:intersectionOf rdf:parseType="Collection">
                    <rdf:Description rdf:about="http://qudt.org/schema/qudt/QuantityValue"/>
                    <owl:Restriction>
                        <owl:onProperty rdf:resource="http://qudt.org/schema/qudt/unit"/>
                        <owl:hasValue rdf:resource="https://qudt.org/3.1.2/vocab/unitDEG"/>
                    </owl:Restriction>
                    <owl:Restriction>
                        <owl:onProperty rdf:resource="http://qudt.org/schema/qudt/numericValue"/>
                        <owl:allValuesFrom>
                            <rdfs:Datatype>
                                <owl:onDatatype rdf:resource="http://www.w3.org/2001/XMLSchema#decimal"/>
                                <owl:withRestrictions rdf:parseType="Collection">
                                    <rdf:Description>
                                        <xsd:minInclusive rdf:datatype="http://www.w3.org/2001/XMLSchema#decimal">0.0</xsd:minInclusive>
                                    </rdf:Description>
                                    <rdf:Description>
                                        <xsd:maxInclusive rdf:datatype="http://www.w3.org/2001/XMLSchema#decimal">360.0</xsd:maxInclusive>
                                    </rdf:Description>
                                </owl:withRestrictions>
                            </rdfs:Datatype>
                        </owl:allValuesFrom>
                    </owl:Restriction>
                </owl:intersectionOf>
            </owl:Class>
        </rdfs:range>
        <rdfs:comment xml:lang="en">Relates a vessel to its course over ground. Indicates the actual course of a vessel over the ground, given as an angle relative to true north (in degrees). Note: This property is semantically the same as http://www.vesselAI-project.eu/ontology#hasCourseOverGround. However, we allow the expression as a quantity with numeric value and a unit.</rdfs:comment>
        <rdfs:label xml:lang="en">has course over ground</rdfs:label>
    </owl:ObjectProperty>
    


    <!-- https://burbachs.github.io/AISHIPOntology/AISHIP#hasDeadweight -->


    <owl:ObjectProperty rdf:about="https://burbachs.github.io/AISHIPOntology/AISHIP#hasDeadweight">
        <rdfs:domain rdf:resource="http://www.vesselAI-project.eu/ontology#Vessel"/>
        <rdfs:range>
            <owl:Class>
                <owl:intersectionOf rdf:parseType="Collection">
                    <rdf:Description rdf:about="http://qudt.org/schema/qudt/QuantityValue"/>
                    <owl:Restriction>
                        <owl:onProperty rdf:resource="http://qudt.org/schema/qudt/unit"/>
                        <owl:hasValue rdf:resource="https://qudt.org/3.1.2/vocab/unitTON_Metric"/>
                    </owl:Restriction>
                    <owl:Restriction>
                        <owl:onProperty rdf:resource="http://qudt.org/schema/qudt/numericValue"/>
                        <owl:allValuesFrom rdf:resource="http://www.w3.org/2001/XMLSchema#decimal"/>
                    </owl:Restriction>
                </owl:intersectionOf>
            </owl:Class>
        </rdfs:range>
        <rdfs:comment xml:lang="en">Relates a vessel to its deadweight. Deadweight tonnage (DWT) represents the maximum weight of cargo, fuel, crew, provisions, and other supplies the vessel can carry, expressed in metric tons. Note: This property is semantically the same as http://www.vesselAI-project.eu/ontology#hasDeadWeight. However, we allow the expression as a quantity with numeric value and a unit.</rdfs:comment>
        <rdfs:label xml:lang="en">has deadweight</rdfs:label>
    </owl:ObjectProperty>
    


    <!-- https://burbachs.github.io/AISHIPOntology/AISHIP#hasDescription -->


    <owl:ObjectProperty rdf:about="https://burbachs.github.io/AISHIPOntology/AISHIP#hasDescription">
        <owl:inverseOf rdf:resource="https://burbachs.github.io/AISHIPOntology/AISHIP#isDescriptionOf"/>
        <rdfs:domain rdf:resource="http://www.vesselAI-project.eu/ontology#Vessel"/>
        <rdfs:range rdf:resource="http://www.semanticdesktop.org/ontologies/2007/03/22/nfo#TextDocument"/>
        <rdfs:comment xml:lang="en">Relates a vessel to its text document description.</rdfs:comment>
        <rdfs:label xml:lang="en">has description</rdfs:label>
    </owl:ObjectProperty>
    


    <!-- https://burbachs.github.io/AISHIPOntology/AISHIP#hasDiameter -->


    <owl:ObjectProperty rdf:about="https://burbachs.github.io/AISHIPOntology/AISHIP#hasDiameter">
        <rdfs:domain rdf:resource="https://burbachs.github.io/AISHIPOntology/AISHIP#BladedPropulsor"/>
        <rdfs:range>
            <owl:Class>
                <owl:intersectionOf rdf:parseType="Collection">
                    <rdf:Description rdf:about="http://qudt.org/schema/qudt/QuantityValue"/>
                    <owl:Restriction>
                        <owl:onProperty rdf:resource="http://qudt.org/schema/qudt/unit"/>
                        <owl:hasValue rdf:resource="https://qudt.org/3.1.2/vocab/unitCentiM"/>
                    </owl:Restriction>
                    <owl:Restriction>
                        <owl:onProperty rdf:resource="http://qudt.org/schema/qudt/numericValue"/>
                        <owl:allValuesFrom rdf:resource="http://www.w3.org/2001/XMLSchema#decimal"/>
                    </owl:Restriction>
                </owl:intersectionOf>
            </owl:Class>
        </rdfs:range>
        <rdfs:comment xml:lang="en">Relates a bladed propulsor to its diameter.</rdfs:comment>
        <rdfs:label xml:lang="en">has diameter</rdfs:label>
    </owl:ObjectProperty>
    


    <!-- https://burbachs.github.io/AISHIPOntology/AISHIP#hasDimensionA -->


    <owl:ObjectProperty rdf:about="https://burbachs.github.io/AISHIPOntology/AISHIP#hasDimensionA">
        <rdfs:domain rdf:resource="http://www.vesselAI-project.eu/ontology#Vessel"/>
        <rdfs:range>
            <owl:Class>
                <owl:intersectionOf rdf:parseType="Collection">
                    <rdf:Description rdf:about="http://qudt.org/schema/qudt/QuantityValue"/>
                    <owl:Restriction>
                        <owl:onProperty rdf:resource="http://qudt.org/schema/qudt/unit"/>
                        <owl:hasValue rdf:resource="https://qudt.org/3.1.2/vocab/unitM"/>
                    </owl:Restriction>
                    <owl:Restriction>
                        <owl:onProperty rdf:resource="http://qudt.org/schema/qudt/numericValue"/>
                        <owl:allValuesFrom rdf:resource="http://www.w3.org/2001/XMLSchema#decimal"/>
                    </owl:Restriction>
                </owl:intersectionOf>
            </owl:Class>
        </rdfs:range>
        <rdfs:comment xml:lang="en">Relates a vessel to its dimension A, i. e. the distance from the GPS antenna to the bow.</rdfs:comment>
        <rdfs:label xml:lang="en">has dimension A</rdfs:label>
    </owl:ObjectProperty>
    


    <!-- https://burbachs.github.io/AISHIPOntology/AISHIP#hasDimensionB -->


    <owl:ObjectProperty rdf:about="https://burbachs.github.io/AISHIPOntology/AISHIP#hasDimensionB">
        <rdfs:domain rdf:resource="http://www.vesselAI-project.eu/ontology#Vessel"/>
        <rdfs:range>
            <owl:Class>
                <owl:intersectionOf rdf:parseType="Collection">
                    <rdf:Description rdf:about="http://qudt.org/schema/qudt/QuantityValue"/>
                    <owl:Restriction>
                        <owl:onProperty rdf:resource="http://qudt.org/schema/qudt/unit"/>
                        <owl:hasValue rdf:resource="https://qudt.org/3.1.2/vocab/unitM"/>
                    </owl:Restriction>
                    <owl:Restriction>
                        <owl:onProperty rdf:resource="http://qudt.org/schema/qudt/numericValue"/>
                        <owl:allValuesFrom rdf:resource="http://www.w3.org/2001/XMLSchema#decimal"/>
                    </owl:Restriction>
                </owl:intersectionOf>
            </owl:Class>
        </rdfs:range>
        <rdfs:comment xml:lang="en">Relates a vessel to its dimension B, i. e. the distance from the GPS antenna to the stern.</rdfs:comment>
        <rdfs:label xml:lang="en">has dimension B</rdfs:label>
    </owl:ObjectProperty>
    


    <!-- https://burbachs.github.io/AISHIPOntology/AISHIP#hasDimensionC -->


    <owl:ObjectProperty rdf:about="https://burbachs.github.io/AISHIPOntology/AISHIP#hasDimensionC">
        <rdfs:domain rdf:resource="http://www.vesselAI-project.eu/ontology#Vessel"/>
        <rdfs:range>
            <owl:Class>
                <owl:intersectionOf rdf:parseType="Collection">
                    <rdf:Description rdf:about="http://qudt.org/schema/qudt/QuantityValue"/>
                    <owl:Restriction>
                        <owl:onProperty rdf:resource="http://qudt.org/schema/qudt/unit"/>
                        <owl:hasValue rdf:resource="https://qudt.org/3.1.2/vocab/unitM"/>
                    </owl:Restriction>
                    <owl:Restriction>
                        <owl:onProperty rdf:resource="http://qudt.org/schema/qudt/numericValue"/>
                        <owl:allValuesFrom rdf:resource="http://www.w3.org/2001/XMLSchema#decimal"/>
                    </owl:Restriction>
                </owl:intersectionOf>
            </owl:Class>
        </rdfs:range>
        <rdfs:comment xml:lang="en">Relates a vessel to its dimension C, i. e. the distance from the GPS antenna to the port side.</rdfs:comment>
        <rdfs:label xml:lang="en">has dimension C</rdfs:label>
    </owl:ObjectProperty>
    


    <!-- https://burbachs.github.io/AISHIPOntology/AISHIP#hasDimensionD -->


    <owl:ObjectProperty rdf:about="https://burbachs.github.io/AISHIPOntology/AISHIP#hasDimensionD">
        <rdfs:domain rdf:resource="http://www.vesselAI-project.eu/ontology#Vessel"/>
        <rdfs:range>
            <owl:Class>
                <owl:intersectionOf rdf:parseType="Collection">
                    <rdf:Description rdf:about="http://qudt.org/schema/qudt/QuantityValue"/>
                    <owl:Restriction>
                        <owl:onProperty rdf:resource="http://qudt.org/schema/qudt/unit"/>
                        <owl:hasValue rdf:resource="https://qudt.org/3.1.2/vocab/unitM"/>
                    </owl:Restriction>
                    <owl:Restriction>
                        <owl:onProperty rdf:resource="http://qudt.org/schema/qudt/numericValue"/>
                        <owl:allValuesFrom rdf:resource="http://www.w3.org/2001/XMLSchema#decimal"/>
                    </owl:Restriction>
                </owl:intersectionOf>
            </owl:Class>
        </rdfs:range>
        <rdfs:comment xml:lang="en">Relates a vessel to its dimension D, i. e. the distance from the GPS antenna to the starboard side.</rdfs:comment>
        <rdfs:label xml:lang="en">has dimension D</rdfs:label>
    </owl:ObjectProperty>
    


    <!-- https://burbachs.github.io/AISHIPOntology/AISHIP#hasDraught -->


    <owl:ObjectProperty rdf:about="https://burbachs.github.io/AISHIPOntology/AISHIP#hasDraught">
        <rdfs:domain rdf:resource="http://www.vesselAI-project.eu/ontology#TrajectoryPart"/>
        <rdfs:range>
            <owl:Class>
                <owl:intersectionOf rdf:parseType="Collection">
                    <rdf:Description rdf:about="http://qudt.org/schema/qudt/QuantityValue"/>
                    <owl:Restriction>
                        <owl:onProperty rdf:resource="http://qudt.org/schema/qudt/unit"/>
                        <owl:hasValue rdf:resource="https://qudt.org/3.1.2/vocab/unitM"/>
                    </owl:Restriction>
                    <owl:Restriction>
                        <owl:onProperty rdf:resource="http://qudt.org/schema/qudt/numericValue"/>
                        <owl:allValuesFrom rdf:resource="http://www.w3.org/2001/XMLSchema#decimal"/>
                    </owl:Restriction>
                </owl:intersectionOf>
            </owl:Class>
        </rdfs:range>
        <rdfs:comment xml:lang="en">Relates a vessel to its draught, i.e., the vertical distance between the waterline and the lowest point of the hull (typically the keel), typically measured in meters (m).</rdfs:comment>
        <rdfs:label xml:lang="en">has draught</rdfs:label>
    </owl:ObjectProperty>
    


    <!-- https://burbachs.github.io/AISHIPOntology/AISHIP#hasGrossTn -->


    <owl:ObjectProperty rdf:about="https://burbachs.github.io/AISHIPOntology/AISHIP#hasGrossTn">
        <rdfs:domain rdf:resource="http://www.vesselAI-project.eu/ontology#Vessel"/>
        <rdfs:range>
            <owl:Class>
                <owl:intersectionOf rdf:parseType="Collection">
                    <rdf:Description rdf:about="http://qudt.org/schema/qudt/QuantityValue"/>
                    <owl:Restriction>
                        <owl:onProperty rdf:resource="http://qudt.org/schema/qudt/unit"/>
                        <owl:hasValue rdf:resource="https://qudt.org/3.1.2/vocab/unitGT"/>
                    </owl:Restriction>
                    <owl:Restriction>
                        <owl:onProperty rdf:resource="http://qudt.org/schema/qudt/numericValue"/>
                        <owl:allValuesFrom rdf:resource="http://www.w3.org/2001/XMLSchema#decimal"/>
                    </owl:Restriction>
                </owl:intersectionOf>
            </owl:Class>
        </rdfs:range>
        <rdfs:comment xml:lang="en">Relates a vessel to its gross tonnage (GT). Indicates the gross tonnage (GT) of the vessel, a dimensionless index defined by the IMO Tonnage Convention based on the ship&apos;s enclosed volume. Note: This property is semantically the same as http://www.vesselAI-project.eu/ontology#hasGrossTn. However, we allow the expression as a quantity with numeric value and a unit.</rdfs:comment>
        <rdfs:label xml:lang="en">has gross tn</rdfs:label>
    </owl:ObjectProperty>
    


    <!-- https://burbachs.github.io/AISHIPOntology/AISHIP#hasHeading -->


    <owl:ObjectProperty rdf:about="https://burbachs.github.io/AISHIPOntology/AISHIP#hasHeading">
        <rdfs:domain rdf:resource="http://www.vesselAI-project.eu/ontology#Vessel"/>
        <rdfs:range>
            <owl:Class>
                <owl:intersectionOf rdf:parseType="Collection">
                    <rdf:Description rdf:about="http://qudt.org/schema/qudt/QuantityValue"/>
                    <owl:Restriction>
                        <owl:onProperty rdf:resource="http://qudt.org/schema/qudt/unit"/>
                        <owl:hasValue rdf:resource="https://qudt.org/3.1.2/vocab/unitDEG"/>
                    </owl:Restriction>
                    <owl:Restriction>
                        <owl:onProperty rdf:resource="http://qudt.org/schema/qudt/numericValue"/>
                        <owl:allValuesFrom>
                            <rdfs:Datatype>
                                <owl:onDatatype rdf:resource="http://www.w3.org/2001/XMLSchema#decimal"/>
                                <owl:withRestrictions rdf:parseType="Collection">
                                    <rdf:Description>
                                        <xsd:minInclusive rdf:datatype="http://www.w3.org/2001/XMLSchema#decimal">0.0</xsd:minInclusive>
                                    </rdf:Description>
                                    <rdf:Description>
                                        <xsd:maxInclusive rdf:datatype="http://www.w3.org/2001/XMLSchema#decimal">360.0</xsd:maxInclusive>
                                    </rdf:Description>
                                </owl:withRestrictions>
                            </rdfs:Datatype>
                        </owl:allValuesFrom>
                    </owl:Restriction>
                </owl:intersectionOf>
            </owl:Class>
        </rdfs:range>
        <rdfs:comment xml:lang="en">Relates a vessel to its heading. Indicates the orientation of the vessel&apos;s bow relative to true or magnetic north, expressed as an angle in degrees. Note: This property is semantically the same as http://www.vesselAI-project.eu/ontology#hasHeading. However, we allow the expression as a quantity with numeric value and a unit.</rdfs:comment>
        <rdfs:label xml:lang="en">has heading</rdfs:label>
    </owl:ObjectProperty>
    


    <!-- https://burbachs.github.io/AISHIPOntology/AISHIP#hasHeight -->


    <owl:ObjectProperty rdf:about="https://burbachs.github.io/AISHIPOntology/AISHIP#hasHeight">
        <rdfs:domain rdf:resource="http://www.vesselAI-project.eu/ontology#Vessel"/>
        <rdfs:range>
            <owl:Class>
                <owl:intersectionOf rdf:parseType="Collection">
                    <rdf:Description rdf:about="http://qudt.org/schema/qudt/QuantityValue"/>
                    <owl:Restriction>
                        <owl:onProperty rdf:resource="http://qudt.org/schema/qudt/unit"/>
                        <owl:hasValue rdf:resource="https://qudt.org/3.1.2/vocab/unitM"/>
                    </owl:Restriction>
                    <owl:Restriction>
                        <owl:onProperty rdf:resource="http://qudt.org/schema/qudt/numericValue"/>
                        <owl:allValuesFrom rdf:resource="http://www.w3.org/2001/XMLSchema#decimal"/>
                    </owl:Restriction>
                </owl:intersectionOf>
            </owl:Class>
        </rdfs:range>
        <rdfs:comment xml:lang="en">Relates a vessel to its height. Indicates the overall height of the vessel, generally from the keel to the highest point, expressed in meters. Note: This property is semantically the same as http://www.vesselAI-project.eu/ontology#hasHeight. However, we allow the expression as a quantity with numeric value and a unit.</rdfs:comment>
        <rdfs:label xml:lang="en">has height</rdfs:label>
    </owl:ObjectProperty>
    


    <!-- https://burbachs.github.io/AISHIPOntology/AISHIP#hasLength -->


    <owl:ObjectProperty rdf:about="https://burbachs.github.io/AISHIPOntology/AISHIP#hasLength">
        <rdfs:domain rdf:resource="http://www.vesselAI-project.eu/ontology#Vessel"/>
        <rdfs:range>
            <owl:Class>
                <owl:intersectionOf rdf:parseType="Collection">
                    <rdf:Description rdf:about="http://qudt.org/schema/qudt/QuantityValue"/>
                    <owl:Restriction>
                        <owl:onProperty rdf:resource="http://qudt.org/schema/qudt/unit"/>
                        <owl:hasValue rdf:resource="https://qudt.org/3.1.2/vocab/unitM"/>
                    </owl:Restriction>
                    <owl:Restriction>
                        <owl:onProperty rdf:resource="http://qudt.org/schema/qudt/numericValue"/>
                        <owl:allValuesFrom rdf:resource="http://www.w3.org/2001/XMLSchema#decimal"/>
                    </owl:Restriction>
                </owl:intersectionOf>
            </owl:Class>
        </rdfs:range>
        <rdfs:comment xml:lang="en">Relates a vessel to its length. Indicates the overall length of the vessel, typically measured in meters. Note: This property is semantically the same as http://www.vesselAI-project.eu/ontology#hasLength. However, we allow the expression as a quantity with numeric value and a unit.</rdfs:comment>
        <rdfs:label xml:lang="en">has length</rdfs:label>
    </owl:ObjectProperty>
    


    <!-- https://burbachs.github.io/AISHIPOntology/AISHIP#hasOwner -->


    <owl:ObjectProperty rdf:about="https://burbachs.github.io/AISHIPOntology/AISHIP#hasOwner">
        <owl:inverseOf rdf:resource="https://burbachs.github.io/AISHIPOntology/AISHIP#isOwnerOf"/>
        <rdfs:domain rdf:resource="http://www.vesselAI-project.eu/ontology#Vessel"/>
        <rdfs:range rdf:resource="https://burbachs.github.io/AISHIPOntology/AISHIP#Owner"/>
        <rdfs:comment xml:lang="en">Relates a vessel to its owner</rdfs:comment>
        <rdfs:label xml:lang="en">has owner</rdfs:label>
    </owl:ObjectProperty>
    


    <!-- https://burbachs.github.io/AISHIPOntology/AISHIP#hasPhoto -->


    <owl:ObjectProperty rdf:about="https://burbachs.github.io/AISHIPOntology/AISHIP#hasPhoto">
        <owl:inverseOf rdf:resource="https://burbachs.github.io/AISHIPOntology/AISHIP#isPhotoOf"/>
        <rdfs:domain rdf:resource="http://www.vesselAI-project.eu/ontology#Vessel"/>
        <rdfs:range rdf:resource="https://www.semanticdesktop.org/ontologies/2007/05/10/nexif/Photo"/>
        <rdfs:comment xml:lang="en">Relates a vessel to its photo.</rdfs:comment>
        <rdfs:label xml:lang="en">has photo</rdfs:label>
    </owl:ObjectProperty>
    


    <!-- https://burbachs.github.io/AISHIPOntology/AISHIP#hasSonarSignature -->


    <owl:ObjectProperty rdf:about="https://burbachs.github.io/AISHIPOntology/AISHIP#hasSonarSignature">
        <owl:inverseOf rdf:resource="https://burbachs.github.io/AISHIPOntology/AISHIP#isSonarSignatureOf"/>
        <rdfs:domain rdf:resource="http://www.vesselAI-project.eu/ontology#Vessel"/>
        <rdfs:range rdf:resource="http://www.semanticdesktop.org/ontologies/2007/03/22/nfo#Audio"/>
        <rdfs:comment xml:lang="en">Relates a vessel to its sonar signature audio file.</rdfs:comment>
        <rdfs:label xml:lang="en">has sonar signature</rdfs:label>
    </owl:ObjectProperty>
    


    <!-- https://burbachs.github.io/AISHIPOntology/AISHIP#hasSpeedOverGround -->


    <owl:ObjectProperty rdf:about="https://burbachs.github.io/AISHIPOntology/AISHIP#hasSpeedOverGround">
        <rdfs:domain rdf:resource="http://www.vesselAI-project.eu/ontology#Vessel"/>
        <rdfs:range>
            <owl:Class>
                <owl:intersectionOf rdf:parseType="Collection">
                    <rdf:Description rdf:about="http://qudt.org/schema/qudt/QuantityValue"/>
                    <owl:Restriction>
                        <owl:onProperty rdf:resource="http://qudt.org/schema/qudt/unit"/>
                        <owl:hasValue rdf:resource="https://qudt.org/3.1.2/vocab/unitKN"/>
                    </owl:Restriction>
                    <owl:Restriction>
                        <owl:onProperty rdf:resource="http://qudt.org/schema/qudt/numericValue"/>
                        <owl:allValuesFrom rdf:resource="http://www.w3.org/2001/XMLSchema#decimal"/>
                    </owl:Restriction>
                </owl:intersectionOf>
            </owl:Class>
        </rdfs:range>
        <rdfs:comment xml:lang="en">Relates a vessel to its speed over ground (SOG). SOG indicates the speed of a vessel relative to the ground surface. Not to be confused with speed through water. Note: This property is semantically the same as http://www.vesselAI-project.eu/ontology#hasSpeedOverGround. However, we allow the expression as a quantity with numeric value and a unit.</rdfs:comment>
        <rdfs:label xml:lang="en">has speed over ground</rdfs:label>
    </owl:ObjectProperty>
    


    <!-- https://burbachs.github.io/AISHIPOntology/AISHIP#hasTypicalGeometry -->


    <owl:ObjectProperty rdf:about="https://burbachs.github.io/AISHIPOntology/AISHIP#hasTypicalGeometry">
        <rdfs:subPropertyOf rdf:resource="http://www.vesselAI-project.eu/ontology#hasGeometry"/>
        <rdfs:domain rdf:resource="https://burbachs.github.io/AISHIPOntology/AISHIP#TypicalLocation"/>
        <rdfs:range rdf:resource="http://www.opengis.net/ont/geosparql#Geometry"/>
        <rdfs:comment xml:lang="en">Relates a typical location of a vessel with its geometry.</rdfs:comment>
        <rdfs:label xml:lang="en">has typical geometry</rdfs:label>
    </owl:ObjectProperty>
    


    <!-- https://burbachs.github.io/AISHIPOntology/AISHIP#hasTypicalLocation -->


    <owl:ObjectProperty rdf:about="https://burbachs.github.io/AISHIPOntology/AISHIP#hasTypicalLocation">
        <rdfs:domain rdf:resource="http://www.vesselAI-project.eu/ontology#Vessel"/>
        <rdfs:range rdf:resource="https://burbachs.github.io/AISHIPOntology/AISHIP#TypicalLocation"/>
        <rdfs:comment xml:lang="en">Related a vessel with its typical location.</rdfs:comment>
        <rdfs:label xml:lang="en">has typical location</rdfs:label>
    </owl:ObjectProperty>
    


    <!-- https://burbachs.github.io/AISHIPOntology/AISHIP#hasWidth -->


    <owl:ObjectProperty rdf:about="https://burbachs.github.io/AISHIPOntology/AISHIP#hasWidth">
        <rdfs:domain rdf:resource="http://www.vesselAI-project.eu/ontology#Vessel"/>
        <rdfs:range>
            <owl:Class>
                <owl:intersectionOf rdf:parseType="Collection">
                    <rdf:Description rdf:about="http://qudt.org/schema/qudt/QuantityValue"/>
                    <owl:Restriction>
                        <owl:onProperty rdf:resource="http://qudt.org/schema/qudt/unit"/>
                        <owl:hasValue rdf:resource="https://qudt.org/3.1.2/vocab/unitM"/>
                    </owl:Restriction>
                    <owl:Restriction>
                        <owl:onProperty rdf:resource="http://qudt.org/schema/qudt/numericValue"/>
                        <owl:allValuesFrom rdf:resource="http://www.w3.org/2001/XMLSchema#decimal"/>
                    </owl:Restriction>
                </owl:intersectionOf>
            </owl:Class>
        </rdfs:range>
        <rdfs:comment xml:lang="en">Relates a vessel to its width. Indicates the overall width (beam) of the vessel, measured in meters. Note: This property is semantically the same as http://www.vesselAI-project.eu/ontology#hasWidth. However, we allow the expression as a quantity with numeric value and a unit.</rdfs:comment>
        <rdfs:label xml:lang="en">has width</rdfs:label>
    </owl:ObjectProperty>
    


    <!-- https://burbachs.github.io/AISHIPOntology/AISHIP#isAntiCavitationMechanismFor -->


    <owl:ObjectProperty rdf:about="https://burbachs.github.io/AISHIPOntology/AISHIP#isAntiCavitationMechanismFor">
        <rdfs:domain rdf:resource="https://burbachs.github.io/AISHIPOntology/AISHIP#AntiCavitationMechanism"/>
        <rdfs:range rdf:resource="https://burbachs.github.io/AISHIPOntology/AISHIP#MotorizedPropulsionTechnology"/>
        <rdfs:comment xml:lang="en">Relates an anti-cavitation mechanism to the motorized propulsion technology it reduces the cavitation of.</rdfs:comment>
        <rdfs:label xml:lang="en">is anti-cavitation mechanism for</rdfs:label>
    </owl:ObjectProperty>
    


    <!-- https://burbachs.github.io/AISHIPOntology/AISHIP#isDescriptionOf -->


    <owl:ObjectProperty rdf:about="https://burbachs.github.io/AISHIPOntology/AISHIP#isDescriptionOf">
        <rdfs:domain rdf:resource="http://www.semanticdesktop.org/ontologies/2007/03/22/nfo#TextDocument"/>
        <rdfs:range rdf:resource="http://www.vesselAI-project.eu/ontology#Vessel"/>
        <rdfs:comment xml:lang="en">Relates a text document description to a vessel</rdfs:comment>
        <rdfs:label xml:lang="en">is description of</rdfs:label>
    </owl:ObjectProperty>
    


    <!-- https://burbachs.github.io/AISHIPOntology/AISHIP#isOwnerOf -->


    <owl:ObjectProperty rdf:about="https://burbachs.github.io/AISHIPOntology/AISHIP#isOwnerOf">
        <rdfs:domain rdf:resource="https://burbachs.github.io/AISHIPOntology/AISHIP#Owner"/>
        <rdfs:range rdf:resource="http://www.vesselAI-project.eu/ontology#Vessel"/>
        <rdfs:comment xml:lang="en">Relates an owner to its vessel.</rdfs:comment>
        <rdfs:label xml:lang="en">is owner of</rdfs:label>
    </owl:ObjectProperty>
    


    <!-- https://burbachs.github.io/AISHIPOntology/AISHIP#isPhotoOf -->


    <owl:ObjectProperty rdf:about="https://burbachs.github.io/AISHIPOntology/AISHIP#isPhotoOf">
        <rdfs:domain rdf:resource="https://www.semanticdesktop.org/ontologies/2007/05/10/nexif/Photo"/>
        <rdfs:range rdf:resource="http://www.vesselAI-project.eu/ontology#Vessel"/>
        <rdfs:comment xml:lang="en">Relates a photo to its vessel.</rdfs:comment>
        <rdfs:label xml:lang="en">is photo of</rdfs:label>
    </owl:ObjectProperty>
    


    <!-- https://burbachs.github.io/AISHIPOntology/AISHIP#isSonarSignatureOf -->


    <owl:ObjectProperty rdf:about="https://burbachs.github.io/AISHIPOntology/AISHIP#isSonarSignatureOf">
        <rdfs:domain rdf:resource="http://www.semanticdesktop.org/ontologies/2007/03/22/nfo#Audio"/>
        <rdfs:range rdf:resource="http://www.vesselAI-project.eu/ontology#Vessel"/>
        <rdfs:comment xml:lang="en">Relates a sonar signature audio file to its vessel.</rdfs:comment>
        <rdfs:label xml:lang="en">is sonar signature of</rdfs:label>
    </owl:ObjectProperty>
    


    <!-- https://burbachs.github.io/AISHIPOntology/AISHIP#poweredBy -->


    <owl:ObjectProperty rdf:about="https://burbachs.github.io/AISHIPOntology/AISHIP#poweredBy">
        <owl:inverseOf rdf:resource="https://burbachs.github.io/AISHIPOntology/AISHIP#powers"/>
        <rdfs:domain rdf:resource="https://schema.org/EngineSpecification"/>
        <rdfs:range rdf:resource="https://burbachs.github.io/AISHIPOntology/AISHIP#PowerGenerationUnit"/>
        <rdfs:comment xml:lang="en">Relates an engine to the power generation unit it is powered by.</rdfs:comment>
        <rdfs:label xml:lang="en">powered by</rdfs:label>
    </owl:ObjectProperty>
    


    <!-- https://burbachs.github.io/AISHIPOntology/AISHIP#powers -->


    <owl:ObjectProperty rdf:about="https://burbachs.github.io/AISHIPOntology/AISHIP#powers">
        <rdfs:domain rdf:resource="https://burbachs.github.io/AISHIPOntology/AISHIP#PowerGenerationUnit"/>
        <rdfs:range rdf:resource="https://schema.org/EngineSpecification"/>
        <rdfs:comment xml:lang="en">Relates a power generation unit to the engine it powers.</rdfs:comment>
        <rdfs:label xml:lang="en">powers</rdfs:label>
    </owl:ObjectProperty>
    


    <!-- https://burbachs.github.io/AISHIPOntology/AISHIP#propelledBy -->


    <owl:ObjectProperty rdf:about="https://burbachs.github.io/AISHIPOntology/AISHIP#propelledBy">
        <owl:inverseOf rdf:resource="https://burbachs.github.io/AISHIPOntology/AISHIP#propells"/>
        <rdfs:domain rdf:resource="http://www.vesselAI-project.eu/ontology#Vessel"/>
        <rdfs:range rdf:resource="https://burbachs.github.io/AISHIPOntology/AISHIP#PropulsionSystem"/>
        <rdfs:comment xml:lang="en">Relates a vessel to the propulsion system it is propelled by.</rdfs:comment>
        <rdfs:label xml:lang="en">propelled by</rdfs:label>
    </owl:ObjectProperty>
    


    <!-- https://burbachs.github.io/AISHIPOntology/AISHIP#propells -->


    <owl:ObjectProperty rdf:about="https://burbachs.github.io/AISHIPOntology/AISHIP#propells">
        <rdfs:domain rdf:resource="https://burbachs.github.io/AISHIPOntology/AISHIP#PropulsionSystem"/>
        <rdfs:range rdf:resource="http://www.vesselAI-project.eu/ontology#Vessel"/>
        <rdfs:comment xml:lang="en">Relates a propulsion system to the vessel it propells.</rdfs:comment>
        <rdfs:label xml:lang="en">propells</rdfs:label>
    </owl:ObjectProperty>
    


    <!-- https://burbachs.github.io/AISHIPOntology/AISHIP#usedByPropulsionSystem -->


    <owl:ObjectProperty rdf:about="https://burbachs.github.io/AISHIPOntology/AISHIP#usedByPropulsionSystem">
        <owl:inverseOf rdf:resource="https://burbachs.github.io/AISHIPOntology/AISHIP#usesPropulsionTechnology"/>
        <rdfs:domain rdf:resource="https://burbachs.github.io/AISHIPOntology/AISHIP#PropulsionTechnology"/>
        <rdfs:range rdf:resource="https://burbachs.github.io/AISHIPOntology/AISHIP#PropulsionSystem"/>
        <rdfs:comment xml:lang="en">Relates a propulsion technology to the propulsion system it is used by to create thrust.</rdfs:comment>
        <rdfs:label xml:lang="en">used by propulsion system</rdfs:label>
    </owl:ObjectProperty>
    


    <!-- https://burbachs.github.io/AISHIPOntology/AISHIP#usesPropulsionTechnology -->


    <owl:ObjectProperty rdf:about="https://burbachs.github.io/AISHIPOntology/AISHIP#usesPropulsionTechnology">
        <rdfs:domain rdf:resource="https://burbachs.github.io/AISHIPOntology/AISHIP#PropulsionSystem"/>
        <rdfs:range rdf:resource="https://burbachs.github.io/AISHIPOntology/AISHIP#PropulsionTechnology"/>
        <rdfs:comment xml:lang="en">Relates a propulsion system to the propulsion technology it uses to create thrust.</rdfs:comment>
        <rdfs:label xml:lang="en">uses propulsion technology</rdfs:label>
    </owl:ObjectProperty>
    


    <!-- 
    ///////////////////////////////////////////////////////////////////////////////////////
    //
    // Data properties
    //
    ///////////////////////////////////////////////////////////////////////////////////////
     -->


    


    <!-- http://qudt.org/schema/qudt/numericValue -->


    <owl:DatatypeProperty rdf:about="http://qudt.org/schema/qudt/numericValue"/>
    


    <!-- https://burbachs.github.io/AISHIPOntology/AISHIP#hasBuiltDate -->


    <owl:DatatypeProperty rdf:about="https://burbachs.github.io/AISHIPOntology/AISHIP#hasBuiltDate">
        <rdfs:domain rdf:resource="http://www.vesselAI-project.eu/ontology#Vessel"/>
        <rdfs:range rdf:resource="http://www.w3.org/2001/XMLSchema#gYear"/>
        <rdfs:comment xml:lang="en">Relates a vessel to the year it was build. Note: This property is semantically the same as http://www.vesselAI-project.eu/ontology#hasBuiltDate. However, we specify the datatype.</rdfs:comment>
        <rdfs:label xml:lang="en">has built date</rdfs:label>
    </owl:DatatypeProperty>
    


    <!-- https://burbachs.github.io/AISHIPOntology/AISHIP#hasHIN -->


    <owl:DatatypeProperty rdf:about="https://burbachs.github.io/AISHIPOntology/AISHIP#hasHIN">
        <rdfs:domain rdf:resource="http://www.vesselAI-project.eu/ontology#Vessel"/>
        <rdfs:range rdf:resource="http://www.w3.org/2001/XMLSchema#string"/>
        <rdfs:comment xml:lang="en">Relates a vessel with its HIN.</rdfs:comment>
        <rdfs:label xml:lang="en">has HIN</rdfs:label>
    </owl:DatatypeProperty>
    


    <!-- https://burbachs.github.io/AISHIPOntology/AISHIP#hasNumberOfBlades -->


    <owl:DatatypeProperty rdf:about="https://burbachs.github.io/AISHIPOntology/AISHIP#hasNumberOfBlades">
        <rdfs:domain rdf:resource="https://burbachs.github.io/AISHIPOntology/AISHIP#BladedPropulsor"/>
        <rdfs:range rdf:resource="http://www.w3.org/2001/XMLSchema#int"/>
        <rdfs:comment xml:lang="en">Relates a bladed propulsor to its number of blades.</rdfs:comment>
        <rdfs:label xml:lang="en">has number of blades</rdfs:label>
    </owl:DatatypeProperty>
    


    <!-- 
    ///////////////////////////////////////////////////////////////////////////////////////
    //
    // Classes
    //
    ///////////////////////////////////////////////////////////////////////////////////////
     -->


    


    <!-- http://qudt.org/schema/qudt/QuantityValue -->


    <owl:Class rdf:about="http://qudt.org/schema/qudt/QuantityValue"/>
    


    <!-- http://www.opengis.net/ont/geosparql#Geometry -->


    <owl:Class rdf:about="http://www.opengis.net/ont/geosparql#Geometry"/>
    


    <!-- http://www.semanticdesktop.org/ontologies/2007/03/22/nfo#Audio -->


    <owl:Class rdf:about="http://www.semanticdesktop.org/ontologies/2007/03/22/nfo#Audio">
        <rdfs:comment xml:lang="en">A file containing an audio content</rdfs:comment>
        <rdfs:label xml:lang="en">Audio</rdfs:label>
    </owl:Class>
    


    <!-- http://www.semanticdesktop.org/ontologies/2007/03/22/nfo#TextDocument -->


    <owl:Class rdf:about="http://www.semanticdesktop.org/ontologies/2007/03/22/nfo#TextDocument">
        <rdfs:comment xml:lang="en">A text document.</rdfs:comment>
        <rdfs:label xml:lang="en">Text document</rdfs:label>
    </owl:Class>
    


    <!-- http://www.vesselAI-project.eu/ontology#Place -->


    <owl:Class rdf:about="http://www.vesselAI-project.eu/ontology#Place"/>
    


    <!-- http://www.vesselAI-project.eu/ontology#SyntheticTrajectory -->


    <owl:Class rdf:about="http://www.vesselAI-project.eu/ontology#SyntheticTrajectory"/>
    


    <!-- http://www.vesselAI-project.eu/ontology#Trajectory -->


    <owl:Class rdf:about="http://www.vesselAI-project.eu/ontology#Trajectory"/>
    


    <!-- http://www.vesselAI-project.eu/ontology#TrajectoryPart -->


    <owl:Class rdf:about="http://www.vesselAI-project.eu/ontology#TrajectoryPart"/>
    


    <!-- http://www.vesselAI-project.eu/ontology#Vessel -->


    <owl:Class rdf:about="http://www.vesselAI-project.eu/ontology#Vessel">
        <rdfs:subClassOf rdf:resource="https://schema.org/Vehicle"/>
        <rdfs:label xml:lang="en">Vessel</rdfs:label>
    </owl:Class>
    


    <!-- http://www.w3.org/2006/time#Interval -->


    <owl:Class rdf:about="http://www.w3.org/2006/time#Interval"/>
    


    <!-- http://xmlns.com/foaf/0.1/Person -->


    <owl:Class rdf:about="http://xmlns.com/foaf/0.1/Person"/>
    


    <!-- https://burbachs.github.io/AISHIPOntology/AISHIP#AntiCavitationMechanism -->


    <owl:Class rdf:about="https://burbachs.github.io/AISHIPOntology/AISHIP#AntiCavitationMechanism">
        <rdfs:comment xml:lang="en">A design feature or technology applied to propulsion systems to prevent or reduce cavitation effects on propeller blades or related components. Such mechanisms aim to minimize efficiency loss, noise, and material damage caused by cavitation.</rdfs:comment>
        <rdfs:label xml:lang="en">Anti cavitation mechanism</rdfs:label>
    </owl:Class>
    


    <!-- https://burbachs.github.io/AISHIPOntology/AISHIP#BatteryUnit -->


    <owl:Class rdf:about="https://burbachs.github.io/AISHIPOntology/AISHIP#BatteryUnit">
        <rdfs:subClassOf rdf:resource="https://burbachs.github.io/AISHIPOntology/AISHIP#PowerGenerationUnit"/>
        <rdfs:comment xml:lang="en">An energy storage system that supplies electrical power for propulsion or auxiliary systems, charged from onboard or external sources.</rdfs:comment>
        <rdfs:label xml:lang="en">Battery unit</rdfs:label>
    </owl:Class>
    


    <!-- https://burbachs.github.io/AISHIPOntology/AISHIP#BladedPropulsor -->


    <owl:Class rdf:about="https://burbachs.github.io/AISHIPOntology/AISHIP#BladedPropulsor">
        <rdfs:subClassOf rdf:resource="https://burbachs.github.io/AISHIPOntology/AISHIP#MotorizedPropulsionTechnology"/>
        <rdfs:comment xml:lang="en">A motorized propulsion technology that generates thrust using rotating blades to accelerate water. This category includes conventional propellers and specialized blade-based systems designed for various operational profiles.</rdfs:comment>
        <rdfs:label xml:lang="en">Bladed propulsor</rdfs:label>
    </owl:Class>
    


    <!-- https://burbachs.github.io/AISHIPOntology/AISHIP#CODAD -->


    <owl:Class rdf:about="https://burbachs.github.io/AISHIPOntology/AISHIP#CODAD">
        <rdfs:subClassOf rdf:resource="https://burbachs.github.io/AISHIPOntology/AISHIP#CombinedEngine"/>
        <rdfs:comment xml:lang="en">A combined propulsion system that uses multiple diesel engines in parallel to provide flexible power management and redundancy.</rdfs:comment>
        <rdfs:label xml:lang="en">CODAD</rdfs:label>
    </owl:Class>
    


    <!-- https://burbachs.github.io/AISHIPOntology/AISHIP#CODAG -->


    <owl:Class rdf:about="https://burbachs.github.io/AISHIPOntology/AISHIP#CODAG">
        <rdfs:subClassOf rdf:resource="https://burbachs.github.io/AISHIPOntology/AISHIP#CombinedEngine"/>
        <rdfs:comment xml:lang="en">A combined propulsion system that can use both a diesel engine and a gas turbine simultaneously for increased power output.</rdfs:comment>
        <rdfs:label xml:lang="en">CODAG</rdfs:label>
    </owl:Class>
    


    <!-- https://burbachs.github.io/AISHIPOntology/AISHIP#CODLAG -->


    <owl:Class rdf:about="https://burbachs.github.io/AISHIPOntology/AISHIP#CODLAG">
        <rdfs:subClassOf rdf:resource="https://burbachs.github.io/AISHIPOntology/AISHIP#CombinedEngine"/>
        <rdfs:comment xml:lang="en">A combined propulsion system that integrates diesel-electric drive for cruising and a gas turbine for greater speed when needed.</rdfs:comment>
        <rdfs:label xml:lang="en">CODLAG</rdfs:label>
    </owl:Class>
    


    <!-- https://burbachs.github.io/AISHIPOntology/AISHIP#CODOG -->


    <owl:Class rdf:about="https://burbachs.github.io/AISHIPOntology/AISHIP#CODOG">
        <rdfs:subClassOf rdf:resource="https://burbachs.github.io/AISHIPOntology/AISHIP#CombinedEngine"/>
        <rdfs:comment xml:lang="en">A combined propulsion system that uses either a diesel engine for efficient cruising or a gas turbine for high-speed operation.</rdfs:comment>
        <rdfs:label xml:lang="en">CODOG</rdfs:label>
    </owl:Class>
    


    <!-- https://burbachs.github.io/AISHIPOntology/AISHIP#COGAG -->


    <owl:Class rdf:about="https://burbachs.github.io/AISHIPOntology/AISHIP#COGAG">
        <rdfs:subClassOf rdf:resource="https://burbachs.github.io/AISHIPOntology/AISHIP#CombinedEngine"/>
        <rdfs:comment xml:lang="en">A combined propulsion system using multiple gas turbines, with smaller units for efficient cruising and additional turbines engaged for high-speed operation.</rdfs:comment>
        <rdfs:label xml:lang="en">COGAG</rdfs:label>
    </owl:Class>
    


    <!-- https://burbachs.github.io/AISHIPOntology/AISHIP#COGAS -->


    <owl:Class rdf:about="https://burbachs.github.io/AISHIPOntology/AISHIP#COGAS">
        <rdfs:subClassOf rdf:resource="https://burbachs.github.io/AISHIPOntology/AISHIP#CombinedEngine"/>
        <rdfs:comment xml:lang="en">A combined propulsion system that integrates a gas turbine and a steam turbine, often in a combined-cycle configuration for efficiency.</rdfs:comment>
        <rdfs:label xml:lang="en">COGAS</rdfs:label>
    </owl:Class>
    


    <!-- https://burbachs.github.io/AISHIPOntology/AISHIP#COGES -->


    <owl:Class rdf:about="https://burbachs.github.io/AISHIPOntology/AISHIP#COGES">
        <rdfs:subClassOf rdf:resource="https://burbachs.github.io/AISHIPOntology/AISHIP#CombinedEngine"/>
        <rdfs:comment xml:lang="en">A combined propulsion system using gas and steam turbines to generate electricity, which powers electric motors for propulsion.</rdfs:comment>
        <rdfs:label xml:lang="en">COGES</rdfs:label>
    </owl:Class>
    


    <!-- https://burbachs.github.io/AISHIPOntology/AISHIP#COGOG -->


    <owl:Class rdf:about="https://burbachs.github.io/AISHIPOntology/AISHIP#COGOG">
        <rdfs:subClassOf rdf:resource="https://burbachs.github.io/AISHIPOntology/AISHIP#CombinedEngine"/>
        <rdfs:comment xml:lang="en">A combined propulsion system with two gas turbines, where only one operates at a time depending on the desired speed profile.</rdfs:comment>
        <rdfs:label xml:lang="en">COGOG</rdfs:label>
    </owl:Class>
    


    <!-- https://burbachs.github.io/AISHIPOntology/AISHIP#CONAG -->


    <owl:Class rdf:about="https://burbachs.github.io/AISHIPOntology/AISHIP#CONAG">
        <rdfs:subClassOf rdf:resource="https://burbachs.github.io/AISHIPOntology/AISHIP#CombinedEngine"/>
        <rdfs:comment xml:lang="en">An experimental propulsion system combining a nuclear reactor with a gas turbine, typically used in advanced naval vessels.</rdfs:comment>
        <rdfs:label xml:lang="en">CONAG</rdfs:label>
    </owl:Class>
    


    <!-- https://burbachs.github.io/AISHIPOntology/AISHIP#CONAN -->


    <owl:Class rdf:about="https://burbachs.github.io/AISHIPOntology/AISHIP#CONAN">
        <rdfs:subClassOf rdf:resource="https://burbachs.github.io/AISHIPOntology/AISHIP#CombinedEngine"/>
        <rdfs:comment xml:lang="en">An experimental propulsion system using two nuclear reactors for increased redundancy and sustained power output.</rdfs:comment>
        <rdfs:label xml:lang="en">CONAN</rdfs:label>
    </owl:Class>
    


    <!-- https://burbachs.github.io/AISHIPOntology/AISHIP#CONAS -->


    <owl:Class rdf:about="https://burbachs.github.io/AISHIPOntology/AISHIP#CONAS">
        <rdfs:subClassOf rdf:resource="https://burbachs.github.io/AISHIPOntology/AISHIP#CombinedEngine"/>
        <rdfs:comment xml:lang="en">A combined propulsion system that uses a nuclear reactor to generate steam, which drives a steam turbine for propulsion.</rdfs:comment>
        <rdfs:label xml:lang="en">CONAS</rdfs:label>
    </owl:Class>
    


    <!-- https://burbachs.github.io/AISHIPOntology/AISHIP#COSAG -->


    <owl:Class rdf:about="https://burbachs.github.io/AISHIPOntology/AISHIP#COSAG">
        <rdfs:subClassOf rdf:resource="https://burbachs.github.io/AISHIPOntology/AISHIP#CombinedEngine"/>
        <rdfs:comment xml:lang="en">A combined propulsion system using a steam turbine for cruising and a gas turbine for rapid acceleration, with optional simultaneous operation.</rdfs:comment>
        <rdfs:label xml:lang="en">COSAG</rdfs:label>
    </owl:Class>
    


    <!-- https://burbachs.github.io/AISHIPOntology/AISHIP#CombinedEngine -->


    <owl:Class rdf:about="https://burbachs.github.io/AISHIPOntology/AISHIP#CombinedEngine">
        <rdfs:subClassOf rdf:resource="https://schema.org/EngineSpecification"/>
        <rdfs:comment xml:lang="en">A propulsion system that integrates two or more engine types to optimize performance, efficiency, or redundancy.</rdfs:comment>
        <rdfs:label xml:lang="en">Combined engine</rdfs:label>
    </owl:Class>
    


    <!-- https://burbachs.github.io/AISHIPOntology/AISHIP#ControllablePitchPropeller -->


    <owl:Class rdf:about="https://burbachs.github.io/AISHIPOntology/AISHIP#ControllablePitchPropeller">
        <rdfs:subClassOf rdf:resource="https://burbachs.github.io/AISHIPOntology/AISHIP#ScrewPropeller"/>
        <rdfs:comment xml:lang="en">A screw propeller with blades that can adjust their pitch during operation, allowing flexible control of thrust and speed without changing the rotation direction. Frequently used in ships that require frequent speed or direction changes.</rdfs:comment>
        <rdfs:label xml:lang="en">Controllable pitch propeller</rdfs:label>
    </owl:Class>
    


    <!-- https://burbachs.github.io/AISHIPOntology/AISHIP#CounterRotatingPropeller -->


    <owl:Class rdf:about="https://burbachs.github.io/AISHIPOntology/AISHIP#CounterRotatingPropeller">
        <rdfs:subClassOf rdf:resource="https://burbachs.github.io/AISHIPOntology/AISHIP#ScrewPropeller"/>
        <rdfs:comment xml:lang="en">A screw propeller system that uses two coaxial propellers rotating in opposite directions to improve efficiency and reduce rotational losses. This design enhances thrust and is typically used on high-performance vessels.</rdfs:comment>
        <rdfs:label xml:lang="en">Counter rotating propeller</rdfs:label>
    </owl:Class>
    


    <!-- https://burbachs.github.io/AISHIPOntology/AISHIP#DieselCombustionUnit -->


    <owl:Class rdf:about="https://burbachs.github.io/AISHIPOntology/AISHIP#DieselCombustionUnit">
        <rdfs:subClassOf rdf:resource="https://burbachs.github.io/AISHIPOntology/AISHIP#PowerGenerationUnit"/>
        <rdfs:comment xml:lang="en">A power unit that generates mechanical or electrical energy by combusting diesel fuel. Often used to drive generators or directly coupled engines.</rdfs:comment>
        <rdfs:label xml:lang="en">Diesel combustion unit</rdfs:label>
    </owl:Class>
    


    <!-- https://burbachs.github.io/AISHIPOntology/AISHIP#DieselEngine -->


    <owl:Class rdf:about="https://burbachs.github.io/AISHIPOntology/AISHIP#DieselEngine">
        <rdfs:subClassOf rdf:resource="https://burbachs.github.io/AISHIPOntology/AISHIP#PistonEngine"/>
        <rdfs:comment xml:lang="en">An internal combustion engine that uses the compression ignition of diesel fuel to produce mechanical motion.</rdfs:comment>
        <rdfs:label xml:lang="en">Diesel engine</rdfs:label>
    </owl:Class>
    


    <!-- https://burbachs.github.io/AISHIPOntology/AISHIP#DuctedPropeller -->


    <owl:Class rdf:about="https://burbachs.github.io/AISHIPOntology/AISHIP#DuctedPropeller">
        <rdfs:subClassOf rdf:resource="https://burbachs.github.io/AISHIPOntology/AISHIP#ScrewPropeller"/>
        <rdfs:comment xml:lang="en">A screw propeller enclosed in a fixed nozzle (duct) to increase thrust and efficiency at lower speeds and provide additional protection. Widely used in tugs and fishing trawlers requiring high bollard pull.</rdfs:comment>
        <rdfs:label xml:lang="en">Ducted propeller</rdfs:label>
    </owl:Class>
    


    <!-- https://burbachs.github.io/AISHIPOntology/AISHIP#ElectricEngine -->


    <owl:Class rdf:about="https://burbachs.github.io/AISHIPOntology/AISHIP#ElectricEngine">
        <rdfs:subClassOf rdf:resource="https://burbachs.github.io/AISHIPOntology/AISHIP#NonPistonEngine"/>
        <rdfs:comment xml:lang="en">A motor that converts electrical energy into mechanical rotation.</rdfs:comment>
        <rdfs:label xml:lang="en">Electric engine</rdfs:label>
    </owl:Class>
    


    <!-- https://burbachs.github.io/AISHIPOntology/AISHIP#FixedPitchPropeller -->


    <owl:Class rdf:about="https://burbachs.github.io/AISHIPOntology/AISHIP#FixedPitchPropeller">
        <rdfs:subClassOf rdf:resource="https://burbachs.github.io/AISHIPOntology/AISHIP#ScrewPropeller"/>
        <rdfs:comment xml:lang="en">A screw propeller with blades fixed at a constant angle. It offers simple and cost-effective design, commonly used in vessels with steady operating conditions where speed and load vary little.</rdfs:comment>
        <rdfs:label xml:lang="en">Fixed pitch propeller</rdfs:label>
    </owl:Class>
    


    <!-- https://burbachs.github.io/AISHIPOntology/AISHIP#FlettnerRotor -->


    <owl:Class rdf:about="https://burbachs.github.io/AISHIPOntology/AISHIP#FlettnerRotor">
        <rdfs:subClassOf rdf:resource="https://burbachs.github.io/AISHIPOntology/AISHIP#RotorSails"/>
        <rdfs:comment xml:lang="en">A specific type of rotor sail consisting of a tall, rotating cylinder mounted vertically on the deck. When wind flows across the spinning surface, lift is generated via the Magnus effect, assisting vessel propulsion.</rdfs:comment>
        <rdfs:label xml:lang="en">Flettner rotor</rdfs:label>
    </owl:Class>
    


    <!-- https://burbachs.github.io/AISHIPOntology/AISHIP#GasCombustionUnit -->


    <owl:Class rdf:about="https://burbachs.github.io/AISHIPOntology/AISHIP#GasCombustionUnit">
        <rdfs:subClassOf rdf:resource="https://burbachs.github.io/AISHIPOntology/AISHIP#PowerGenerationUnit"/>
        <rdfs:comment xml:lang="en">A power unit that burns gaseous fuels such as natural gas or LNG to produce usable energy for shipboard systems or propulsion.</rdfs:comment>
        <rdfs:label xml:lang="en">Gas combustion unit</rdfs:label>
    </owl:Class>
    


    <!-- https://burbachs.github.io/AISHIPOntology/AISHIP#GasTurbineEngine -->


    <owl:Class rdf:about="https://burbachs.github.io/AISHIPOntology/AISHIP#GasTurbineEngine">
        <rdfs:subClassOf rdf:resource="https://burbachs.github.io/AISHIPOntology/AISHIP#NonPistonEngine"/>
        <rdfs:comment xml:lang="en">A rotary engine that generates mechanical power by expanding combustion gases through turbine stages.</rdfs:comment>
        <rdfs:label xml:lang="en">Gas turbine engine</rdfs:label>
    </owl:Class>
    


    <!-- https://burbachs.github.io/AISHIPOntology/AISHIP#GasWaterJet -->


    <owl:Class rdf:about="https://burbachs.github.io/AISHIPOntology/AISHIP#GasWaterJet">
        <rdfs:subClassOf rdf:resource="https://burbachs.github.io/AISHIPOntology/AISHIP#JetPropulsor"/>
        <rdfs:comment xml:lang="en">A jet propulsion technology that uses gas (e.g., exhaust gases from a turbine) instead of a pumpt to accelerate water and create thrust. This system combines combustion energy with fluid dynamics for high-performance propulsion.</rdfs:comment>
        <rdfs:label xml:lang="en">Gas-water jet</rdfs:label>
    </owl:Class>
    


    <!-- https://burbachs.github.io/AISHIPOntology/AISHIP#HardSail -->


    <owl:Class rdf:about="https://burbachs.github.io/AISHIPOntology/AISHIP#HardSail">
        <rdfs:subClassOf rdf:resource="https://burbachs.github.io/AISHIPOntology/AISHIP#Sail"/>
        <rdfs:comment xml:lang="en">A rigid sail structure, typically resembling an aerofoil, used to harness wind energy for propulsion.</rdfs:comment>
        <rdfs:label xml:lang="en">Hard sail</rdfs:label>
    </owl:Class>
    


    <!-- https://burbachs.github.io/AISHIPOntology/AISHIP#HullForm -->


    <owl:Class rdf:about="https://burbachs.github.io/AISHIPOntology/AISHIP#HullForm">
        <rdfs:subClassOf rdf:resource="https://burbachs.github.io/AISHIPOntology/AISHIP#WindAssistedPropulsionTechnology"/>
        <rdfs:comment xml:lang="en">A wind-assisted propulsion technology that utilizes the vessel’s hull geometry to generate additional aerodynamic lift or reduce drag, complementing primary propulsion systems.</rdfs:comment>
        <rdfs:label xml:lang="en">Hull form</rdfs:label>
    </owl:Class>
    


    <!-- https://burbachs.github.io/AISHIPOntology/AISHIP#JetPropulsor -->


    <owl:Class rdf:about="https://burbachs.github.io/AISHIPOntology/AISHIP#JetPropulsor">
        <rdfs:subClassOf rdf:resource="https://burbachs.github.io/AISHIPOntology/AISHIP#MotorizedPropulsionTechnology"/>
        <rdfs:comment xml:lang="en">A motorized propulsion technology that generates thrust by accelerating a fluid (typically water) through a nozzle, creating a jet stream that propels the vessel. Jet propulsors are commonly used for high-speed boats and specialized vessels.</rdfs:comment>
        <rdfs:label xml:lang="en">Jet propulsor</rdfs:label>
    </owl:Class>
    


    <!-- https://burbachs.github.io/AISHIPOntology/AISHIP#Kite -->


    <owl:Class rdf:about="https://burbachs.github.io/AISHIPOntology/AISHIP#Kite">
        <rdfs:subClassOf rdf:resource="https://burbachs.github.io/AISHIPOntology/AISHIP#WindAssistedPropulsionTechnology"/>
        <rdfs:comment xml:lang="en">A wind-assisted propulsion technology that uses a large controllable kite deployed ahead of the vessel to harness wind energy and reduce engine power requirements.</rdfs:comment>
        <rdfs:label xml:lang="en">Kite</rdfs:label>
    </owl:Class>
    


    <!-- https://burbachs.github.io/AISHIPOntology/AISHIP#MotorizedPropulsionSystem -->


    <owl:Class rdf:about="https://burbachs.github.io/AISHIPOntology/AISHIP#MotorizedPropulsionSystem">
        <rdfs:subClassOf rdf:resource="https://burbachs.github.io/AISHIPOntology/AISHIP#PropulsionSystem"/>
        <rdfs:subClassOf>
            <owl:Restriction>
                <owl:onProperty rdf:resource="https://burbachs.github.io/AISHIPOntology/AISHIP#usesPropulsionTechnology"/>
                <owl:allValuesFrom rdf:resource="https://burbachs.github.io/AISHIPOntology/AISHIP#MotorizedPropulsionTechnology"/>
            </owl:Restriction>
        </rdfs:subClassOf>
        <owl:disjointWith rdf:resource="https://burbachs.github.io/AISHIPOntology/AISHIP#MusclePoweredPropulsionSystem"/>
        <owl:disjointWith rdf:resource="https://burbachs.github.io/AISHIPOntology/AISHIP#PureWindPropulsionSystem"/>
        <owl:disjointWith rdf:resource="https://burbachs.github.io/AISHIPOntology/AISHIP#WindAssistedPropulsionSystem"/>
        <rdfs:comment xml:lang="en">A propulsion system that relies on internal or external motors or engines to generate mechanical thrust for vessel movement.</rdfs:comment>
        <rdfs:label xml:lang="en">Motorized propulsion system</rdfs:label>
    </owl:Class>
    


    <!-- https://burbachs.github.io/AISHIPOntology/AISHIP#MotorizedPropulsionTechnology -->


    <owl:Class rdf:about="https://burbachs.github.io/AISHIPOntology/AISHIP#MotorizedPropulsionTechnology">
        <rdfs:subClassOf rdf:resource="https://burbachs.github.io/AISHIPOntology/AISHIP#PropulsionTechnology"/>
        <rdfs:subClassOf>
            <owl:Restriction>
                <owl:onProperty rdf:resource="https://burbachs.github.io/AISHIPOntology/AISHIP#usedByPropulsionSystem"/>
                <owl:allValuesFrom rdf:resource="https://burbachs.github.io/AISHIPOntology/AISHIP#MotorizedPropulsionSystem"/>
            </owl:Restriction>
        </rdfs:subClassOf>
        <owl:disjointWith rdf:resource="https://burbachs.github.io/AISHIPOntology/AISHIP#MusclePoweredPropulsionTechnology"/>
        <owl:disjointWith rdf:resource="https://burbachs.github.io/AISHIPOntology/AISHIP#PureWindPropulsionTechnology"/>
        <owl:disjointWith rdf:resource="https://burbachs.github.io/AISHIPOntology/AISHIP#WindAssistedPropulsionTechnology"/>
        <rdfs:comment xml:lang="en">A propulsion technology that relies on mechanical motors or engine to convert energy into thrust for vessel propulsion.</rdfs:comment>
        <rdfs:label xml:lang="en">Motorized propulsion technology</rdfs:label>
    </owl:Class>
    


    <!-- https://burbachs.github.io/AISHIPOntology/AISHIP#MusclePoweredPropulsionSystem -->


    <owl:Class rdf:about="https://burbachs.github.io/AISHIPOntology/AISHIP#MusclePoweredPropulsionSystem">
        <rdfs:subClassOf rdf:resource="https://burbachs.github.io/AISHIPOntology/AISHIP#NonMotorizedPropulsionSystem"/>
        <rdfs:subClassOf>
            <owl:Restriction>
                <owl:onProperty rdf:resource="https://burbachs.github.io/AISHIPOntology/AISHIP#usesPropulsionTechnology"/>
                <owl:allValuesFrom rdf:resource="https://burbachs.github.io/AISHIPOntology/AISHIP#MusclePoweredPropulsionTechnology"/>
            </owl:Restriction>
        </rdfs:subClassOf>
        <owl:disjointWith rdf:resource="https://burbachs.github.io/AISHIPOntology/AISHIP#PureWindPropulsionSystem"/>
        <owl:disjointWith rdf:resource="https://burbachs.github.io/AISHIPOntology/AISHIP#WindAssistedPropulsionSystem"/>
        <rdfs:comment xml:lang="en">A non-motorized propulsion system that generates thrust through human or animal muscular effort, such as rowing with paddles or pedaling mechanisms.</rdfs:comment>
        <rdfs:label xml:lang="en">Muscle-powered propulsion system</rdfs:label>
    </owl:Class>
    


    <!-- https://burbachs.github.io/AISHIPOntology/AISHIP#MusclePoweredPropulsionTechnology -->


    <owl:Class rdf:about="https://burbachs.github.io/AISHIPOntology/AISHIP#MusclePoweredPropulsionTechnology">
        <rdfs:subClassOf rdf:resource="https://burbachs.github.io/AISHIPOntology/AISHIP#PropulsionTechnology"/>
        <rdfs:subClassOf>
            <owl:Restriction>
                <owl:onProperty rdf:resource="https://burbachs.github.io/AISHIPOntology/AISHIP#usedByPropulsionSystem"/>
                <owl:allValuesFrom rdf:resource="https://burbachs.github.io/AISHIPOntology/AISHIP#MusclePoweredPropulsionSystem"/>
            </owl:Restriction>
        </rdfs:subClassOf>
        <owl:disjointWith rdf:resource="https://burbachs.github.io/AISHIPOntology/AISHIP#PureWindPropulsionTechnology"/>
        <owl:disjointWith rdf:resource="https://burbachs.github.io/AISHIPOntology/AISHIP#WindAssistedPropulsionTechnology"/>
        <rdfs:comment xml:lang="en">A type of propulsion method based on human or animal muscular effort, which is applied by a muscle powered propulsion system to generate thrust. Examples include paddling, rowing, or pedaling, depending on the mechanical realization.</rdfs:comment>
        <rdfs:label xml:lang="en">Muscle-powered propulsion technology</rdfs:label>
    </owl:Class>
    


    <!-- https://burbachs.github.io/AISHIPOntology/AISHIP#NonMotorizedPropulsionSystem -->


    <owl:Class rdf:about="https://burbachs.github.io/AISHIPOntology/AISHIP#NonMotorizedPropulsionSystem">
        <rdfs:subClassOf rdf:resource="https://burbachs.github.io/AISHIPOntology/AISHIP#PropulsionSystem"/>
        <rdfs:comment xml:lang="en">A propulsion system that does not employ mechanical motors or engines, typically relying on natural forces or manual input such as wind or muscle power.</rdfs:comment>
        <rdfs:label xml:lang="en">Non-motorized propulsion system</rdfs:label>
    </owl:Class>
    


    <!-- https://burbachs.github.io/AISHIPOntology/AISHIP#NonPistonEngine -->


    <owl:Class rdf:about="https://burbachs.github.io/AISHIPOntology/AISHIP#NonPistonEngine">
        <rdfs:subClassOf rdf:resource="https://schema.org/EngineSpecification"/>
        <rdfs:comment xml:lang="en">An engine that generates mechanical power without using pistons, typically through continuous rotational systems such as turbines or electric motors.</rdfs:comment>
        <rdfs:label xml:lang="en">Non-piston engine</rdfs:label>
    </owl:Class>
    


    <!-- https://burbachs.github.io/AISHIPOntology/AISHIP#NuclearReactor -->


    <owl:Class rdf:about="https://burbachs.github.io/AISHIPOntology/AISHIP#NuclearReactor">
        <rdfs:subClassOf rdf:resource="https://burbachs.github.io/AISHIPOntology/AISHIP#PowerGenerationUnit"/>
        <rdfs:comment xml:lang="en">A reactor that generates thermal energy through controlled nuclear fission, typically used to power steam turbines in naval or large-scale vessels.</rdfs:comment>
        <rdfs:label xml:lang="en">Nuclear reactor</rdfs:label>
    </owl:Class>
    


    <!-- https://burbachs.github.io/AISHIPOntology/AISHIP#Owner -->


    <owl:Class rdf:about="https://burbachs.github.io/AISHIPOntology/AISHIP#Owner">
        <rdfs:comment xml:lang="en">The owner of a vessel.</rdfs:comment>
        <rdfs:label xml:lang="en">Owner</rdfs:label>
    </owl:Class>
    


    <!-- https://burbachs.github.io/AISHIPOntology/AISHIP#Paddle -->


    <owl:Class rdf:about="https://burbachs.github.io/AISHIPOntology/AISHIP#Paddle">
        <rdfs:subClassOf rdf:resource="https://burbachs.github.io/AISHIPOntology/AISHIP#MusclePoweredPropulsionTechnology"/>
        <rdfs:comment xml:lang="en">A simple muscle-powered propulsion technique involving a handheld blade used to push against water and move a vessel forward. Typically associated with canoes, kayaks, or lifeboats.</rdfs:comment>
        <rdfs:label xml:lang="en">Paddle</rdfs:label>
    </owl:Class>
    


    <!-- https://burbachs.github.io/AISHIPOntology/AISHIP#PaddleWheel -->


    <owl:Class rdf:about="https://burbachs.github.io/AISHIPOntology/AISHIP#PaddleWheel">
        <rdfs:subClassOf rdf:resource="https://burbachs.github.io/AISHIPOntology/AISHIP#BladedPropulsor"/>
        <rdfs:comment xml:lang="en">A propulsion technology that uses large external wheels with attached blades or paddles to push water and generate thrust. Historically used in riverboats and still applied in some shallow-water or heritage vessels.</rdfs:comment>
        <rdfs:label xml:lang="en">Paddle wheel</rdfs:label>
    </owl:Class>
    


    <!-- https://burbachs.github.io/AISHIPOntology/AISHIP#PistonEngine -->


    <owl:Class rdf:about="https://burbachs.github.io/AISHIPOntology/AISHIP#PistonEngine">
        <rdfs:subClassOf rdf:resource="https://schema.org/EngineSpecification"/>
        <rdfs:comment xml:lang="en">An internal combustion engine that converts the linear motion of pistons into rotational energy via a crankshaft.</rdfs:comment>
        <rdfs:label xml:lang="en">Piston engine</rdfs:label>
    </owl:Class>
    


    <!-- https://burbachs.github.io/AISHIPOntology/AISHIP#PowerGenerationUnit -->


    <owl:Class rdf:about="https://burbachs.github.io/AISHIPOntology/AISHIP#PowerGenerationUnit">
        <rdfs:comment xml:lang="en">A power unit that produces usable energy for shipboard systems or propulsion.</rdfs:comment>
        <rdfs:label xml:lang="en">Power generation unit</rdfs:label>
    </owl:Class>
    


    <!-- https://burbachs.github.io/AISHIPOntology/AISHIP#PredictedTrajectory -->


    <owl:Class rdf:about="https://burbachs.github.io/AISHIPOntology/AISHIP#PredictedTrajectory">
        <rdfs:subClassOf rdf:resource="http://www.vesselAI-project.eu/ontology#SyntheticTrajectory"/>
        <rdfs:comment xml:lang="en">A trajectory that is predicted based on the analysis of previous vessel trajectories.</rdfs:comment>
        <rdfs:label xml:lang="en">Predicted trajectory</rdfs:label>
    </owl:Class>
    


    <!-- https://burbachs.github.io/AISHIPOntology/AISHIP#PropellerPod -->


    <owl:Class rdf:about="https://burbachs.github.io/AISHIPOntology/AISHIP#PropellerPod">
        <rdfs:subClassOf rdf:resource="https://burbachs.github.io/AISHIPOntology/AISHIP#SpeciallyDesignedBladedPropulsor"/>
        <rdfs:comment xml:lang="en">A propulsion system where the propeller is mounted on a steerable pod that also contains the drive motor. Podded propulsors allow full 360-degree rotation for excellent maneuverability and are commonly used in cruise ships and offshore vessels.</rdfs:comment>
        <rdfs:label xml:lang="en">Propeller pod</rdfs:label>
    </owl:Class>
    


    <!-- https://burbachs.github.io/AISHIPOntology/AISHIP#PropulsionSystem -->


    <owl:Class rdf:about="https://burbachs.github.io/AISHIPOntology/AISHIP#PropulsionSystem">
        <rdfs:comment xml:lang="en">A system that generates thrust to move a vessel forward.</rdfs:comment>
        <rdfs:label xml:lang="en">Propulsion system</rdfs:label>
    </owl:Class>
    


    <!-- https://burbachs.github.io/AISHIPOntology/AISHIP#PropulsionTechnology -->


    <owl:Class rdf:about="https://burbachs.github.io/AISHIPOntology/AISHIP#PropulsionTechnology">
        <rdfs:comment xml:lang="en">A general concept representing the method or technology used by a propulsion system to generate thrust for vessel movement. This class provides an abstraction for different approaches such as motor-driven or wind-based techniques.</rdfs:comment>
        <rdfs:label xml:lang="en">Propulsion technology</rdfs:label>
    </owl:Class>
    


    <!-- https://burbachs.github.io/AISHIPOntology/AISHIP#PureWindHardSail -->


    <owl:Class rdf:about="https://burbachs.github.io/AISHIPOntology/AISHIP#PureWindHardSail">
        <rdfs:subClassOf rdf:resource="https://burbachs.github.io/AISHIPOntology/AISHIP#HardSail"/>
        <rdfs:subClassOf rdf:resource="https://burbachs.github.io/AISHIPOntology/AISHIP#PureWindPropulsionTechnology"/>
        <rdfs:comment xml:lang="en">A rigid sail designed to provide the primary propulsion for a vessel using wind energy alone.</rdfs:comment>
        <rdfs:label xml:lang="en">Pure wind hard sail</rdfs:label>
    </owl:Class>
    


    <!-- https://burbachs.github.io/AISHIPOntology/AISHIP#PureWindPropulsionSystem -->


    <owl:Class rdf:about="https://burbachs.github.io/AISHIPOntology/AISHIP#PureWindPropulsionSystem">
        <rdfs:subClassOf rdf:resource="https://burbachs.github.io/AISHIPOntology/AISHIP#NonMotorizedPropulsionSystem"/>
        <rdfs:subClassOf>
            <owl:Restriction>
                <owl:onProperty rdf:resource="https://burbachs.github.io/AISHIPOntology/AISHIP#usesPropulsionTechnology"/>
                <owl:allValuesFrom rdf:resource="https://burbachs.github.io/AISHIPOntology/AISHIP#PureWindPropulsionTechnology"/>
            </owl:Restriction>
        </rdfs:subClassOf>
        <owl:disjointWith rdf:resource="https://burbachs.github.io/AISHIPOntology/AISHIP#WindAssistedPropulsionSystem"/>
        <rdfs:comment xml:lang="en">A propulsion system that exclusively uses wind energy, captured via sails or other aerodynamic surfaces, to generate forward thrust without auxiliary engines.</rdfs:comment>
        <rdfs:label xml:lang="en">Pure wind propulsion system</rdfs:label>
    </owl:Class>
    


    <!-- https://burbachs.github.io/AISHIPOntology/AISHIP#PureWindPropulsionTechnology -->


    <owl:Class rdf:about="https://burbachs.github.io/AISHIPOntology/AISHIP#PureWindPropulsionTechnology">
        <rdfs:subClassOf rdf:resource="https://burbachs.github.io/AISHIPOntology/AISHIP#PropulsionTechnology"/>
        <rdfs:subClassOf>
            <owl:Restriction>
                <owl:onProperty rdf:resource="https://burbachs.github.io/AISHIPOntology/AISHIP#usedByPropulsionSystem"/>
                <owl:allValuesFrom rdf:resource="https://burbachs.github.io/AISHIPOntology/AISHIP#PureWindPropulsionSystem"/>
            </owl:Restriction>
        </rdfs:subClassOf>
        <owl:disjointWith rdf:resource="https://burbachs.github.io/AISHIPOntology/AISHIP#WindAssistedPropulsionTechnology"/>
        <rdfs:comment xml:lang="en">A wind propulsion technology that exclusively uses wind as the energy source for generating thrust, without assistance from motorized systems. Typical implementation involves sails or other aerodynamic devices.</rdfs:comment>
        <rdfs:label xml:lang="en">Pure wind propulsion technology</rdfs:label>
    </owl:Class>
    


    <!-- https://burbachs.github.io/AISHIPOntology/AISHIP#PureWindSoftSail -->


    <owl:Class rdf:about="https://burbachs.github.io/AISHIPOntology/AISHIP#PureWindSoftSail">
        <rdfs:subClassOf rdf:resource="https://burbachs.github.io/AISHIPOntology/AISHIP#PureWindPropulsionTechnology"/>
        <rdfs:subClassOf rdf:resource="https://burbachs.github.io/AISHIPOntology/AISHIP#SoftSail"/>
        <rdfs:comment xml:lang="en">A traditional or modern soft sail used to provide the primary propulsion for a vessel using wind energy alone.</rdfs:comment>
        <rdfs:label xml:lang="en">Pure wind soft sail</rdfs:label>
    </owl:Class>
    


    <!-- https://burbachs.github.io/AISHIPOntology/AISHIP#RestrictedArea -->


    <owl:Class rdf:about="https://burbachs.github.io/AISHIPOntology/AISHIP#RestrictedArea">
        <rdfs:subClassOf rdf:resource="http://www.vesselAI-project.eu/ontology#Place"/>
        <rdfs:comment xml:lang="en">A maritime region where access or navigation is limited due to security, safety, or legal regulations.</rdfs:comment>
        <rdfs:label xml:lang="en">Restricted area</rdfs:label>
    </owl:Class>
    


    <!-- https://burbachs.github.io/AISHIPOntology/AISHIP#RotorSails -->


    <owl:Class rdf:about="https://burbachs.github.io/AISHIPOntology/AISHIP#RotorSails">
        <rdfs:subClassOf rdf:resource="https://burbachs.github.io/AISHIPOntology/AISHIP#WindAssistedPropulsionTechnology"/>
        <rdfs:comment xml:lang="en">A wind-assisted propulsion technology that uses rotating cylindrical sails (rotors) to create aerodynamic lift through the Magnus effect, reducing engine load and fuel consumption.</rdfs:comment>
        <rdfs:label xml:lang="en">Rotor sails</rdfs:label>
    </owl:Class>
    


    <!-- https://burbachs.github.io/AISHIPOntology/AISHIP#RudderPropeller -->


    <owl:Class rdf:about="https://burbachs.github.io/AISHIPOntology/AISHIP#RudderPropeller">
        <rdfs:subClassOf rdf:resource="https://burbachs.github.io/AISHIPOntology/AISHIP#ScrewPropeller"/>
        <rdfs:comment xml:lang="en">A screw propeller integrated with a steerable drive unit, enabling both propulsion and steering without a separate rudder. Common in azimuth thrusters for offshore vessels and ships needing high maneuverability.</rdfs:comment>
        <rdfs:label xml:lang="en">Rudder propeller</rdfs:label>
    </owl:Class>
    


    <!-- https://burbachs.github.io/AISHIPOntology/AISHIP#Sail -->


    <owl:Class rdf:about="https://burbachs.github.io/AISHIPOntology/AISHIP#Sail">
        <rdfs:comment xml:lang="en">A generic sail that converts wind energy into propulsive force for a vessel.</rdfs:comment>
        <rdfs:label xml:lang="en">Sail</rdfs:label>
    </owl:Class>
    


    <!-- https://burbachs.github.io/AISHIPOntology/AISHIP#ScrewPropeller -->


    <owl:Class rdf:about="https://burbachs.github.io/AISHIPOntology/AISHIP#ScrewPropeller">
        <rdfs:subClassOf rdf:resource="https://burbachs.github.io/AISHIPOntology/AISHIP#BladedPropulsor"/>
        <rdfs:comment xml:lang="en">A widely used bladed propulsion technology where helical blades mounted on a rotating hub create thrust by pushing water backwards. Screw propellers are commonly used for most vessel types due to their simplicity and efficiency.</rdfs:comment>
        <rdfs:label xml:lang="en">Screw propeller</rdfs:label>
    </owl:Class>
    


    <!-- https://burbachs.github.io/AISHIPOntology/AISHIP#SoftSail -->


    <owl:Class rdf:about="https://burbachs.github.io/AISHIPOntology/AISHIP#SoftSail">
        <rdfs:subClassOf rdf:resource="https://burbachs.github.io/AISHIPOntology/AISHIP#Sail"/>
        <rdfs:comment xml:lang="en">A flexible sail made from fabric or similar materials, traditionally used for harnessing wind energy.</rdfs:comment>
        <rdfs:label xml:lang="en">Soft sail</rdfs:label>
    </owl:Class>
    


    <!-- https://burbachs.github.io/AISHIPOntology/AISHIP#SolarArray -->


    <owl:Class rdf:about="https://burbachs.github.io/AISHIPOntology/AISHIP#SolarArray">
        <rdfs:subClassOf rdf:resource="https://burbachs.github.io/AISHIPOntology/AISHIP#PowerGenerationUnit"/>
        <rdfs:comment xml:lang="en">A photovoltaic system that converts solar radiation into electrical energy, typically used as a supplementary or auxiliary power source.</rdfs:comment>
        <rdfs:label xml:lang="en">Solar array</rdfs:label>
    </owl:Class>
    


    <!-- https://burbachs.github.io/AISHIPOntology/AISHIP#SpeciallyDesignedBladedPropulsor -->


    <owl:Class rdf:about="https://burbachs.github.io/AISHIPOntology/AISHIP#SpeciallyDesignedBladedPropulsor">
        <rdfs:subClassOf rdf:resource="https://burbachs.github.io/AISHIPOntology/AISHIP#BladedPropulsor"/>
        <rdfs:comment xml:lang="en">A bladed propulsion technology adapted for specific vessel requirements or operational conditions, such as high maneuverability or integrated drive systems.</rdfs:comment>
        <rdfs:label xml:lang="en">Specially designed bladed propeller</rdfs:label>
    </owl:Class>
    


    <!-- https://burbachs.github.io/AISHIPOntology/AISHIP#SteamTurbineEngine -->


    <owl:Class rdf:about="https://burbachs.github.io/AISHIPOntology/AISHIP#SteamTurbineEngine">
        <rdfs:subClassOf rdf:resource="https://burbachs.github.io/AISHIPOntology/AISHIP#NonPistonEngine"/>
        <rdfs:comment xml:lang="en">A rotary engine that converts thermal energy from pressurized steam into mechanical motion via rotating turbine blades.</rdfs:comment>
        <rdfs:label xml:lang="en">Steam turbine engine</rdfs:label>
    </owl:Class>
    


    <!-- https://burbachs.github.io/AISHIPOntology/AISHIP#SuctionWings -->


    <owl:Class rdf:about="https://burbachs.github.io/AISHIPOntology/AISHIP#SuctionWings">
        <rdfs:subClassOf rdf:resource="https://burbachs.github.io/AISHIPOntology/AISHIP#WindAssistedPropulsionTechnology"/>
        <rdfs:comment xml:lang="en">A wind-assisted propulsion technology using rigid wing structures with suction or airflow control systems to enhance aerodynamic lift and reduce fuel consumption.</rdfs:comment>
        <rdfs:label xml:lang="en">Suction wings</rdfs:label>
    </owl:Class>
    


    <!-- https://burbachs.github.io/AISHIPOntology/AISHIP#SupercavitatingPropeller -->


    <owl:Class rdf:about="https://burbachs.github.io/AISHIPOntology/AISHIP#SupercavitatingPropeller">
        <rdfs:subClassOf rdf:resource="https://burbachs.github.io/AISHIPOntology/AISHIP#ScrewPropeller"/>
        <rdfs:comment xml:lang="en">A screw propeller designed to operate under conditions of intentional cavitation, reducing drag at very high speeds. Common in fast military or racing vessels where conventional propellers would suffer performance loss.</rdfs:comment>
        <rdfs:label xml:lang="en">Supercavitating propeller</rdfs:label>
    </owl:Class>
    


    <!-- https://burbachs.github.io/AISHIPOntology/AISHIP#TypicalLocation -->


    <owl:Class rdf:about="https://burbachs.github.io/AISHIPOntology/AISHIP#TypicalLocation">
        <rdfs:comment xml:lang="en">The typical location of a vessel that is calculated over a time interval.</rdfs:comment>
        <rdfs:label xml:lang="en">Typical location</rdfs:label>
    </owl:Class>
    


    <!-- https://burbachs.github.io/AISHIPOntology/AISHIP#VesselWithMotorizedPropulsionSystem -->


    <owl:Class rdf:about="https://burbachs.github.io/AISHIPOntology/AISHIP#VesselWithMotorizedPropulsionSystem">
        <owl:equivalentClass>
            <owl:Class>
                <owl:intersectionOf rdf:parseType="Collection">
                    <rdf:Description rdf:about="http://www.vesselAI-project.eu/ontology#Vessel"/>
                    <owl:Restriction>
                        <owl:onProperty rdf:resource="https://burbachs.github.io/AISHIPOntology/AISHIP#propelledBy"/>
                        <owl:someValuesFrom rdf:resource="https://burbachs.github.io/AISHIPOntology/AISHIP#MotorizedPropulsionSystem"/>
                    </owl:Restriction>
                </owl:intersectionOf>
            </owl:Class>
        </owl:equivalentClass>
        <owl:disjointWith rdf:resource="https://burbachs.github.io/AISHIPOntology/AISHIP#VesselWithPureWindPropulsionSystem"/>
        <rdfs:comment xml:lang="en">A vessel that is motorized cannot also be classified as having a pure wind propulsion system.</rdfs:comment>
        <rdfs:comment xml:lang="en">Represents any vessel that has at least one motorized propulsion system.</rdfs:comment>
    </owl:Class>
    


    <!-- https://burbachs.github.io/AISHIPOntology/AISHIP#VesselWithMusclePoweredPropulsionSystem -->


    <owl:Class rdf:about="https://burbachs.github.io/AISHIPOntology/AISHIP#VesselWithMusclePoweredPropulsionSystem">
        <owl:equivalentClass>
            <owl:Class>
                <owl:intersectionOf rdf:parseType="Collection">
                    <rdf:Description rdf:about="http://www.vesselAI-project.eu/ontology#Vessel"/>
                    <owl:Restriction>
                        <owl:onProperty rdf:resource="https://burbachs.github.io/AISHIPOntology/AISHIP#propelledBy"/>
                        <owl:someValuesFrom rdf:resource="https://burbachs.github.io/AISHIPOntology/AISHIP#MusclePoweredPropulsionSystem"/>
                    </owl:Restriction>
                </owl:intersectionOf>
            </owl:Class>
        </owl:equivalentClass>
        <rdfs:comment xml:lang="en">Represents any vessel that has at least one muscle-powered propulsion system.</rdfs:comment>
    </owl:Class>
    


    <!-- https://burbachs.github.io/AISHIPOntology/AISHIP#VesselWithPureWindPropulsionSystem -->


    <owl:Class rdf:about="https://burbachs.github.io/AISHIPOntology/AISHIP#VesselWithPureWindPropulsionSystem">
        <owl:equivalentClass>
            <owl:Class>
                <owl:intersectionOf rdf:parseType="Collection">
                    <rdf:Description rdf:about="http://www.vesselAI-project.eu/ontology#Vessel"/>
                    <owl:Restriction>
                        <owl:onProperty rdf:resource="https://burbachs.github.io/AISHIPOntology/AISHIP#propelledBy"/>
                        <owl:someValuesFrom rdf:resource="https://burbachs.github.io/AISHIPOntology/AISHIP#PureWindPropulsionSystem"/>
                    </owl:Restriction>
                    <owl:Restriction>
                        <owl:onProperty rdf:resource="https://burbachs.github.io/AISHIPOntology/AISHIP#propelledBy"/>
                        <owl:allValuesFrom rdf:resource="https://burbachs.github.io/AISHIPOntology/AISHIP#PureWindPropulsionSystem"/>
                    </owl:Restriction>
                </owl:intersectionOf>
            </owl:Class>
        </owl:equivalentClass>
        <owl:disjointWith rdf:resource="https://burbachs.github.io/AISHIPOntology/AISHIP#VesselWithWindAssistedPropulsionSystem"/>
        <rdfs:comment xml:lang="en">Represents any vessel that has at least one pure wind propulsion system. These kinds of vessel are purely propulled by wind.</rdfs:comment>
    </owl:Class>
    


    <!-- https://burbachs.github.io/AISHIPOntology/AISHIP#VesselWithWindAssistedPropulsionSystem -->


    <owl:Class rdf:about="https://burbachs.github.io/AISHIPOntology/AISHIP#VesselWithWindAssistedPropulsionSystem">
        <owl:equivalentClass>
            <owl:Class>
                <owl:intersectionOf rdf:parseType="Collection">
                    <rdf:Description rdf:about="http://www.vesselAI-project.eu/ontology#Vessel"/>
                    <owl:Restriction>
                        <owl:onProperty rdf:resource="https://burbachs.github.io/AISHIPOntology/AISHIP#propelledBy"/>
                        <owl:someValuesFrom rdf:resource="https://burbachs.github.io/AISHIPOntology/AISHIP#WindAssistedPropulsionSystem"/>
                    </owl:Restriction>
                </owl:intersectionOf>
            </owl:Class>
        </owl:equivalentClass>
        <rdfs:subClassOf>
            <owl:Restriction>
                <owl:onProperty rdf:resource="https://burbachs.github.io/AISHIPOntology/AISHIP#propelledBy"/>
                <owl:someValuesFrom rdf:resource="https://burbachs.github.io/AISHIPOntology/AISHIP#MotorizedPropulsionSystem"/>
            </owl:Restriction>
        </rdfs:subClassOf>
        <rdfs:comment xml:lang="en">A vessel that is wind-assisted cannot also be classified as having a pure wind propulsion system.</rdfs:comment>
        <rdfs:comment xml:lang="en">Represents any vessel that has at least one wind-assisted propulsion system and is required to also have a motorized propulsion system, as wind-assisted systems are intended to supplement motorized propulsion.</rdfs:comment>
    </owl:Class>
    


    <!-- https://burbachs.github.io/AISHIPOntology/AISHIP#VoithSchneiderPropeller -->


    <owl:Class rdf:about="https://burbachs.github.io/AISHIPOntology/AISHIP#VoithSchneiderPropeller">
        <rdfs:subClassOf rdf:resource="https://burbachs.github.io/AISHIPOntology/AISHIP#SpeciallyDesignedBladedPropulsor"/>
        <rdfs:comment xml:lang="en">A highly maneuverable bladed propulsion system using vertical blades that rotate and adjust their pitch cyclically. This design enables precise control in all directions, making it ideal for tugs, ferries, and vessels operating in confined waters.</rdfs:comment>
        <rdfs:label xml:lang="en">Voith Schneider Propeller</rdfs:label>
    </owl:Class>
    


    <!-- https://burbachs.github.io/AISHIPOntology/AISHIP#WaterJet -->


    <owl:Class rdf:about="https://burbachs.github.io/AISHIPOntology/AISHIP#WaterJet">
        <rdfs:subClassOf rdf:resource="https://burbachs.github.io/AISHIPOntology/AISHIP#JetPropulsor"/>
        <rdfs:comment xml:lang="en">A jet propulsion technology that draws water into an intake and expels it at high velocity through a nozzle to generate thrust. Water jets are widely used for high-speed ferries, jet boats, and shallow-water applications.</rdfs:comment>
        <rdfs:label xml:lang="en">Water jet</rdfs:label>
    </owl:Class>
    


    <!-- https://burbachs.github.io/AISHIPOntology/AISHIP#WindAssistedHardSail -->


    <owl:Class rdf:about="https://burbachs.github.io/AISHIPOntology/AISHIP#WindAssistedHardSail">
        <rdfs:subClassOf rdf:resource="https://burbachs.github.io/AISHIPOntology/AISHIP#HardSail"/>
        <rdfs:subClassOf rdf:resource="https://burbachs.github.io/AISHIPOntology/AISHIP#WindAssistedPropulsionTechnology"/>
        <rdfs:comment xml:lang="en">A rigid sail used to supplement the main propulsion system, reducing fuel consumption by utilizing wind energy.</rdfs:comment>
        <rdfs:label xml:lang="en">Wind-assisted hard sail</rdfs:label>
    </owl:Class>
    


    <!-- https://burbachs.github.io/AISHIPOntology/AISHIP#WindAssistedPropulsionSystem -->


    <owl:Class rdf:about="https://burbachs.github.io/AISHIPOntology/AISHIP#WindAssistedPropulsionSystem">
        <rdfs:subClassOf rdf:resource="https://burbachs.github.io/AISHIPOntology/AISHIP#NonMotorizedPropulsionSystem"/>
        <rdfs:subClassOf>
            <owl:Restriction>
                <owl:onProperty rdf:resource="https://burbachs.github.io/AISHIPOntology/AISHIP#usesPropulsionTechnology"/>
                <owl:allValuesFrom rdf:resource="https://burbachs.github.io/AISHIPOntology/AISHIP#WindAssistedPropulsionTechnology"/>
            </owl:Restriction>
        </rdfs:subClassOf>
        <rdfs:comment xml:lang="en">A hybrid propulsion system that supplements motorized thrust with aerodynamic lift generated from wind-driven devices, such as rotor sails, suction wings, or kite sails.</rdfs:comment>
        <rdfs:label>Wind-assisted propulsion system</rdfs:label>
    </owl:Class>
    


    <!-- https://burbachs.github.io/AISHIPOntology/AISHIP#WindAssistedPropulsionTechnology -->


    <owl:Class rdf:about="https://burbachs.github.io/AISHIPOntology/AISHIP#WindAssistedPropulsionTechnology">
        <rdfs:subClassOf rdf:resource="https://burbachs.github.io/AISHIPOntology/AISHIP#PropulsionTechnology"/>
        <rdfs:subClassOf>
            <owl:Restriction>
                <owl:onProperty rdf:resource="https://burbachs.github.io/AISHIPOntology/AISHIP#usedByPropulsionSystem"/>
                <owl:allValuesFrom rdf:resource="https://burbachs.github.io/AISHIPOntology/AISHIP#WindAssistedPropulsionSystem"/>
            </owl:Restriction>
        </rdfs:subClassOf>
        <rdfs:comment xml:lang="en">A hybrid propulsion technology where wind energy supplements motorized propulsion to reduce fuel consumption and improve efficiency. Examples include rotor sails, suction wings, or kites.</rdfs:comment>
        <rdfs:label xml:lang="en">Wind-assisted propulsion technology</rdfs:label>
    </owl:Class>
    


    <!-- https://burbachs.github.io/AISHIPOntology/AISHIP#WindAssistedSoftSail -->


    <owl:Class rdf:about="https://burbachs.github.io/AISHIPOntology/AISHIP#WindAssistedSoftSail">
        <rdfs:subClassOf rdf:resource="https://burbachs.github.io/AISHIPOntology/AISHIP#SoftSail"/>
        <rdfs:subClassOf rdf:resource="https://burbachs.github.io/AISHIPOntology/AISHIP#WindAssistedPropulsionTechnology"/>
        <rdfs:comment xml:lang="en">A flexible sail used to supplement the main propulsion system, reducing fuel consumption by utilizing wind energy.</rdfs:comment>
        <rdfs:label xml:lang="en">Wind-assisted soft sail</rdfs:label>
    </owl:Class>
    


    <!-- https://burbachs.github.io/AISHIPOntology/AISHIP#WindTurbine -->


    <owl:Class rdf:about="https://burbachs.github.io/AISHIPOntology/AISHIP#WindTurbine">
        <rdfs:subClassOf rdf:resource="https://burbachs.github.io/AISHIPOntology/AISHIP#WindAssistedPropulsionTechnology"/>
        <rdfs:comment xml:lang="en">A wind-assisted propulsion technology using rotor blades similar to wind power generators, converting wind energy into thrust or auxiliary electrical energy for propulsion.</rdfs:comment>
        <rdfs:label xml:lang="en">Wind turbine</rdfs:label>
    </owl:Class>
    


    <!-- https://schema.org/EngineSpecification -->


    <owl:Class rdf:about="https://schema.org/EngineSpecification">
        <rdfs:comment xml:lang="en">Information about the engine of the vehicle. A vehicle can have multiple engines represented by multiple engine specification entities.</rdfs:comment>
        <rdfs:label xml:lang="en">Engine specification</rdfs:label>
    </owl:Class>
    


    <!-- https://schema.org/Organization -->


    <owl:Class rdf:about="https://schema.org/Organization">
        <rdfs:subClassOf rdf:resource="https://burbachs.github.io/AISHIPOntology/AISHIP#Owner"/>
        <rdfs:comment xml:lang="en">An organization such as a school, NGO, corporation, club, etc.</rdfs:comment>
        <rdfs:label xml:lang="en">Organization</rdfs:label>
    </owl:Class>
    


    <!-- https://schema.org/Person -->


    <owl:Class rdf:about="https://schema.org/Person">
        <rdfs:subClassOf rdf:resource="https://burbachs.github.io/AISHIPOntology/AISHIP#Owner"/>
        <rdfs:comment xml:lang="en">A person (alive, dead, undead, or fictional).</rdfs:comment>
        <rdfs:label xml:lang="en">Person</rdfs:label>
    </owl:Class>
    


    <!-- https://schema.org/Vehicle -->


    <owl:Class rdf:about="https://schema.org/Vehicle">
        <rdfs:comment xml:lang="en">A vehicle is a device that is designed or used to transport people or cargo over land, water, air, or through space.</rdfs:comment>
        <rdfs:label xml:lang="en">Vehicle</rdfs:label>
    </owl:Class>
    


    <!-- https://www.semanticdesktop.org/ontologies/2007/05/10/nexif/Photo -->


    <owl:Class rdf:about="https://www.semanticdesktop.org/ontologies/2007/05/10/nexif/Photo">
        <rdfs:comment xml:lang="en">A photo, an image captured using a camera, an EXIF Image File Directory.</rdfs:comment>
        <rdfs:label xml:lang="en">Photo</rdfs:label>
    </owl:Class>
    


    <!-- 
    ///////////////////////////////////////////////////////////////////////////////////////
    //
    // Individuals
    //
    ///////////////////////////////////////////////////////////////////////////////////////
     -->


    


    <!-- https://qudt.org/3.1.2/vocab/unitCentiM -->


    <owl:NamedIndividual rdf:about="https://qudt.org/3.1.2/vocab/unitCentiM"/>
    


    <!-- https://qudt.org/3.1.2/vocab/unitDEG -->


    <owl:NamedIndividual rdf:about="https://qudt.org/3.1.2/vocab/unitDEG"/>
    


    <!-- https://qudt.org/3.1.2/vocab/unitGT -->


    <owl:NamedIndividual rdf:about="https://qudt.org/3.1.2/vocab/unitGT"/>
    


    <!-- https://qudt.org/3.1.2/vocab/unitKN -->


    <owl:NamedIndividual rdf:about="https://qudt.org/3.1.2/vocab/unitKN"/>
    


    <!-- https://qudt.org/3.1.2/vocab/unitM -->


    <owl:NamedIndividual rdf:about="https://qudt.org/3.1.2/vocab/unitM"/>
    


    <!-- https://qudt.org/3.1.2/vocab/unitTON_Metric -->


    <owl:NamedIndividual rdf:about="https://qudt.org/3.1.2/vocab/unitTON_Metric"/>
</rdf:RDF>



<!-- Generated by the OWL API (version 5.1.18) https://github.com/owlcs/owlapi/ -->


